Challenge/Modexp/Submission/Proofs/Fast/Paths/CsubFixed.lean
@@ -17,1055 +17,1055 @@ private theorem instructionPC_succ
     assembleBytes_cons, assembleBytes_nil, List.append_nil, List.length_append]
 
 def csGenericPath : List (Challenge.EvmProof.Stepper.Located Artifact.submissionArtifact .Osaka) :=
-  [opAt 3400 .JUMPDEST,
-   pushAt 3401 2 2688,
-   opAt 3402 .MLOAD,
-   pushAt 3403 2 256,
-   opAt 3404 .EQ,
-   pushAt 3405 2 4535,
-   opAt 3406 .JUMPI,
-   pushAt 3407 2 2688,
-   opAt 3408 .MLOAD,
-   pushAt 3409 1 128,
-   opAt 3410 .EQ,
-   pushAt 3411 2 4351,
-   opAt 3412 .JUMPI,
-   pushAt 3413 2 2784,
-   opAt 3414 .MLOAD,
-   pushAt 3415 2 2752,
-   opAt 3416 .MLOAD,
-   opAt 3417 (.Dup ⟨0, by decide⟩),
-   pushAt 3418 2 1792,
-   opAt 3419 .ADD,
-   opAt 3420 (.Swap ⟨0, by decide⟩),
-   pushAt 3421 0 0,
-   opAt 3422 (.Swap ⟨2, by decide⟩),
-   pushAt 3423 2 1561,
-   opAt 3424 .JUMP]
+  [opAt 3397 .JUMPDEST,
+   pushAt 3398 2 2688,
+   opAt 3399 .MLOAD,
+   pushAt 3400 2 256,
+   opAt 3401 .EQ,
+   pushAt 3402 2 4545,
+   opAt 3403 .JUMPI,
+   pushAt 3404 2 2688,
+   opAt 3405 .MLOAD,
+   pushAt 3406 1 128,
+   opAt 3407 .EQ,
+   pushAt 3408 2 4346,
+   opAt 3409 .JUMPI,
+   pushAt 3410 2 2784,
+   opAt 3411 .MLOAD,
+   pushAt 3412 2 2752,
+   opAt 3413 .MLOAD,
+   opAt 3414 (.Dup ⟨0, by decide⟩),
+   pushAt 3415 2 1792,
+   opAt 3416 .ADD,
+   opAt 3417 (.Swap ⟨0, by decide⟩),
+   pushAt 3418 0 0,
+   opAt 3419 (.Swap ⟨2, by decide⟩),
+   pushAt 3420 2 1562,
+   opAt 3421 .JUMP]
 
 def csFixedEntry8 : List (Challenge.EvmProof.Stepper.Located Artifact.submissionArtifact .Osaka) :=
-  [opAt 3400 .JUMPDEST,
-   pushAt 3401 2 2688,
-   opAt 3402 .MLOAD,
-   pushAt 3403 2 256,
-   opAt 3404 .EQ,
-   pushAt 3405 2 4535,
-   opAt 3406 .JUMPI,
-   opAt 3425 .JUMPDEST]
+  [opAt 3397 .JUMPDEST,
+   pushAt 3398 2 2688,
+   opAt 3399 .MLOAD,
+   pushAt 3400 2 256,
+   opAt 3401 .EQ,
+   pushAt 3402 2 4545,
+   opAt 3403 .JUMPI,
+   opAt 3422 .JUMPDEST]
 
 def csFixedEntry4 : List (Challenge.EvmProof.Stepper.Located Artifact.submissionArtifact .Osaka) :=
-  [opAt 3400 .JUMPDEST,
-   pushAt 3401 2 2688,
-   opAt 3402 .MLOAD,
-   pushAt 3403 2 256,
-   opAt 3404 .EQ,
-   pushAt 3405 2 4535,
-   opAt 3406 .JUMPI,
-   pushAt 3407 2 2688,
-   opAt 3408 .MLOAD,
-   pushAt 3409 1 128,
-   opAt 3410 .EQ,
-   pushAt 3411 2 4351,
-   opAt 3412 .JUMPI,
-   opAt 3299 .JUMPDEST]
+  [opAt 3397 .JUMPDEST,
+   pushAt 3398 2 2688,
+   opAt 3399 .MLOAD,
+   pushAt 3400 2 256,
+   opAt 3401 .EQ,
+   pushAt 3402 2 4545,
+   opAt 3403 .JUMPI,
+   pushAt 3404 2 2688,
+   opAt 3405 .MLOAD,
+   pushAt 3406 1 128,
+   opAt 3407 .EQ,
+   pushAt 3408 2 4346,
+   opAt 3409 .JUMPI,
+   opAt 3287 .JUMPDEST]
 
 def csFixedStep8_0 : List (Challenge.EvmProof.Stepper.Located Artifact.submissionArtifact .Osaka) :=
-  [pushAt 3426 2 2336,
-   opAt 3427 .MLOAD,
-   pushAt 3428 1 224,
-   opAt 3429 .MLOAD,
-   opAt 3430 (.Dup ⟨1, by decide⟩),
-   opAt 3431 (.Dup ⟨1, by decide⟩),
-   opAt 3432 .GT,
-   opAt 3433 (.Swap ⟨1, by decide⟩),
-   opAt 3434 .SUB,
-   pushAt 3435 2 2016,
-   opAt 3436 .MSTORE]
+  [pushAt 3423 2 2336,
+   opAt 3424 .MLOAD,
+   pushAt 3425 1 224,
+   opAt 3426 .MLOAD,
+   opAt 3427 (.Dup ⟨1, by decide⟩),
+   opAt 3428 (.Dup ⟨1, by decide⟩),
+   opAt 3429 .GT,
+   opAt 3430 (.Swap ⟨1, by decide⟩),
+   opAt 3431 .SUB,
+   pushAt 3432 2 2016,
+   opAt 3433 .MSTORE]
 
 def csFixedStep8_1 : List (Challenge.EvmProof.Stepper.Located Artifact.submissionArtifact .Osaka) :=
-  [pushAt 3437 2 2304,
-   opAt 3438 .MLOAD,
-   pushAt 3439 1 192,
-   opAt 3440 .MLOAD,
-   opAt 3441 (.Dup ⟨1, by decide⟩),
-   opAt 3442 (.Dup ⟨1, by decide⟩),
-   opAt 3443 .GT,
-   opAt 3444 (.Swap ⟨1, by decide⟩),
+  [pushAt 3434 2 2304,
+   opAt 3435 .MLOAD,
+   pushAt 3436 1 192,
+   opAt 3437 .MLOAD,
+   opAt 3438 (.Dup ⟨1, by decide⟩),
+   opAt 3439 (.Dup ⟨1, by decide⟩),
+   opAt 3440 .GT,
+   opAt 3441 (.Swap ⟨1, by decide⟩),
+   opAt 3442 .SUB,
+   opAt 3443 (.Dup ⟨2, by decide⟩),
+   opAt 3444 (.Dup ⟨1, by decide⟩),
    opAt 3445 .SUB,
-   opAt 3446 (.Dup ⟨2, by decide⟩),
-   opAt 3447 (.Dup ⟨1, by decide⟩),
-   opAt 3448 .SUB,
-   opAt 3449 (.Swap ⟨2, by decide⟩),
-   opAt 3450 .GT,
-   opAt 3451 .OR,
-   opAt 3452 (.Swap ⟨0, by decide⟩),
-   pushAt 3453 2 1984,
-   opAt 3454 .MSTORE]
+   opAt 3446 (.Swap ⟨2, by decide⟩),
+   opAt 3447 .GT,
+   opAt 3448 .OR,
+   opAt 3449 (.Swap ⟨0, by decide⟩),
+   pushAt 3450 2 1984,
+   opAt 3451 .MSTORE]
 
 def csFixedStep8_2 : List (Challenge.EvmProof.Stepper.Located Artifact.submissionArtifact .Osaka) :=
-  [pushAt 3455 2 2272,
-   opAt 3456 .MLOAD,
-   pushAt 3457 1 160,
-   opAt 3458 .MLOAD,
-   opAt 3459 (.Dup ⟨1, by decide⟩),
-   opAt 3460 (.Dup ⟨1, by decide⟩),
-   opAt 3461 .GT,
-   opAt 3462 (.Swap ⟨1, by decide⟩),
+  [pushAt 3452 2 2272,
+   opAt 3453 .MLOAD,
+   pushAt 3454 1 160,
+   opAt 3455 .MLOAD,
+   opAt 3456 (.Dup ⟨1, by decide⟩),
+   opAt 3457 (.Dup ⟨1, by decide⟩),
+   opAt 3458 .GT,
+   opAt 3459 (.Swap ⟨1, by decide⟩),
+   opAt 3460 .SUB,
+   opAt 3461 (.Dup ⟨2, by decide⟩),
+   opAt 3462 (.Dup ⟨1, by decide⟩),
    opAt 3463 .SUB,
-   opAt 3464 (.Dup ⟨2, by decide⟩),
-   opAt 3465 (.Dup ⟨1, by decide⟩),
-   opAt 3466 .SUB,
-   opAt 3467 (.Swap ⟨2, by decide⟩),
-   opAt 3468 .GT,
-   opAt 3469 .OR,
-   opAt 3470 (.Swap ⟨0, by decide⟩),
-   pushAt 3471 2 1952,
-   opAt 3472 .MSTORE]
+   opAt 3464 (.Swap ⟨2, by decide⟩),
+   opAt 3465 .GT,
+   opAt 3466 .OR,
+   opAt 3467 (.Swap ⟨0, by decide⟩),
+   pushAt 3468 2 1952,
+   opAt 3469 .MSTORE]
 
 def csFixedStep8_3 : List (Challenge.EvmProof.Stepper.Located Artifact.submissionArtifact .Osaka) :=
-  [pushAt 3473 2 2240,
-   opAt 3474 .MLOAD,
-   pushAt 3475 1 128,
-   opAt 3476 .MLOAD,
-   opAt 3477 (.Dup ⟨1, by decide⟩),
-   opAt 3478 (.Dup ⟨1, by decide⟩),
-   opAt 3479 .GT,
-   opAt 3480 (.Swap ⟨1, by decide⟩),
+  [pushAt 3470 2 2240,
+   opAt 3471 .MLOAD,
+   pushAt 3472 1 128,
+   opAt 3473 .MLOAD,
+   opAt 3474 (.Dup ⟨1, by decide⟩),
+   opAt 3475 (.Dup ⟨1, by decide⟩),
+   opAt 3476 .GT,
+   opAt 3477 (.Swap ⟨1, by decide⟩),
+   opAt 3478 .SUB,
+   opAt 3479 (.Dup ⟨2, by decide⟩),
+   opAt 3480 (.Dup ⟨1, by decide⟩),
    opAt 3481 .SUB,
-   opAt 3482 (.Dup ⟨2, by decide⟩),
-   opAt 3483 (.Dup ⟨1, by decide⟩),
-   opAt 3484 .SUB,
-   opAt 3485 (.Swap ⟨2, by decide⟩),
-   opAt 3486 .GT,
-   opAt 3487 .OR,
-   opAt 3488 (.Swap ⟨0, by decide⟩),
-   pushAt 3489 2 1920,
-   opAt 3490 .MSTORE]
+   opAt 3482 (.Swap ⟨2, by decide⟩),
+   opAt 3483 .GT,
+   opAt 3484 .OR,
+   opAt 3485 (.Swap ⟨0, by decide⟩),
+   pushAt 3486 2 1920,
+   opAt 3487 .MSTORE]
 
 def csFixedStep8_4 : List (Challenge.EvmProof.Stepper.Located Artifact.submissionArtifact .Osaka) :=
-  [pushAt 3491 2 2208,
-   opAt 3492 .MLOAD,
-   pushAt 3493 1 96,
-   opAt 3494 .MLOAD,
-   opAt 3495 (.Dup ⟨1, by decide⟩),
-   opAt 3496 (.Dup ⟨1, by decide⟩),
-   opAt 3497 .GT,
-   opAt 3498 (.Swap ⟨1, by decide⟩),
+  [pushAt 3488 2 2208,
+   opAt 3489 .MLOAD,
+   pushAt 3490 1 96,
+   opAt 3491 .MLOAD,
+   opAt 3492 (.Dup ⟨1, by decide⟩),
+   opAt 3493 (.Dup ⟨1, by decide⟩),
+   opAt 3494 .GT,
+   opAt 3495 (.Swap ⟨1, by decide⟩),
+   opAt 3496 .SUB,
+   opAt 3497 (.Dup ⟨2, by decide⟩),
+   opAt 3498 (.Dup ⟨1, by decide⟩),
    opAt 3499 .SUB,
-   opAt 3500 (.Dup ⟨2, by decide⟩),
-   opAt 3501 (.Dup ⟨1, by decide⟩),
-   opAt 3502 .SUB,
-   opAt 3503 (.Swap ⟨2, by decide⟩),
-   opAt 3504 .GT,
-   opAt 3505 .OR,
-   opAt 3506 (.Swap ⟨0, by decide⟩),
-   pushAt 3507 2 1888,
-   opAt 3508 .MSTORE]
+   opAt 3500 (.Swap ⟨2, by decide⟩),
+   opAt 3501 .GT,
+   opAt 3502 .OR,
+   opAt 3503 (.Swap ⟨0, by decide⟩),
+   pushAt 3504 2 1888,
+   opAt 3505 .MSTORE]
 
 def csFixedStep8_5 : List (Challenge.EvmProof.Stepper.Located Artifact.submissionArtifact .Osaka) :=
-  [opAt 3509 .JUMPDEST,
-   pushAt 3510 2 2176,
-   opAt 3511 .MLOAD,
-   pushAt 3512 1 64,
-   opAt 3513 .MLOAD,
-   opAt 3514 (.Dup ⟨1, by decide⟩),
-   opAt 3515 (.Dup ⟨1, by decide⟩),
-   opAt 3516 .GT,
-   opAt 3517 (.Swap ⟨1, by decide⟩),
+  [opAt 3506 .JUMPDEST,
+   pushAt 3507 2 2176,
+   opAt 3508 .MLOAD,
+   pushAt 3509 1 64,
+   opAt 3510 .MLOAD,
+   opAt 3511 (.Dup ⟨1, by decide⟩),
+   opAt 3512 (.Dup ⟨1, by decide⟩),
+   opAt 3513 .GT,
+   opAt 3514 (.Swap ⟨1, by decide⟩),
+   opAt 3515 .SUB,
+   opAt 3516 (.Dup ⟨2, by decide⟩),
+   opAt 3517 (.Dup ⟨1, by decide⟩),
    opAt 3518 .SUB,
-   opAt 3519 (.Dup ⟨2, by decide⟩),
-   opAt 3520 (.Dup ⟨1, by decide⟩),
-   opAt 3521 .SUB,
-   opAt 3522 (.Swap ⟨2, by decide⟩),
-   opAt 3523 .GT,
-   opAt 3524 .OR,
-   opAt 3525 (.Swap ⟨0, by decide⟩),
-   pushAt 3526 2 1856,
-   opAt 3527 .MSTORE]
+   opAt 3519 (.Swap ⟨2, by decide⟩),
+   opAt 3520 .GT,
+   opAt 3521 .OR,
+   opAt 3522 (.Swap ⟨0, by decide⟩),
+   pushAt 3523 2 1856,
+   opAt 3524 .MSTORE]
 
 def csFixedStep8_6 : List (Challenge.EvmProof.Stepper.Located Artifact.submissionArtifact .Osaka) :=
-  [pushAt 3528 2 2144,
-   opAt 3529 .MLOAD,
-   pushAt 3530 1 32,
-   opAt 3531 .MLOAD,
-   opAt 3532 (.Dup ⟨1, by decide⟩),
-   opAt 3533 (.Dup ⟨1, by decide⟩),
-   opAt 3534 .GT,
-   opAt 3535 (.Swap ⟨1, by decide⟩),
+  [pushAt 3525 2 2144,
+   opAt 3526 .MLOAD,
+   pushAt 3527 1 32,
+   opAt 3528 .MLOAD,
+   opAt 3529 (.Dup ⟨1, by decide⟩),
+   opAt 3530 (.Dup ⟨1, by decide⟩),
+   opAt 3531 .GT,
+   opAt 3532 (.Swap ⟨1, by decide⟩),
+   opAt 3533 .SUB,
+   opAt 3534 (.Dup ⟨2, by decide⟩),
+   opAt 3535 (.Dup ⟨1, by decide⟩),
    opAt 3536 .SUB,
-   opAt 3537 (.Dup ⟨2, by decide⟩),
-   opAt 3538 (.Dup ⟨1, by decide⟩),
-   opAt 3539 .SUB,
-   opAt 3540 (.Swap ⟨2, by decide⟩),
-   opAt 3541 .GT,
-   opAt 3542 .OR,
-   opAt 3543 (.Swap ⟨0, by decide⟩),
-   pushAt 3544 2 1824,
-   opAt 3545 .MSTORE]
+   opAt 3537 (.Swap ⟨2, by decide⟩),
+   opAt 3538 .GT,
+   opAt 3539 .OR,
+   opAt 3540 (.Swap ⟨0, by decide⟩),
+   pushAt 3541 2 1824,
+   opAt 3542 .MSTORE]
 
 def csFixedStep8_7 : List (Challenge.EvmProof.Stepper.Located Artifact.submissionArtifact .Osaka) :=
-  [pushAt 3546 2 2112,
-   opAt 3547 .MLOAD,
-   pushAt 3548 0 0,
-   opAt 3549 .MLOAD,
-   opAt 3550 (.Dup ⟨1, by decide⟩),
-   opAt 3551 (.Dup ⟨1, by decide⟩),
-   opAt 3552 .GT,
-   opAt 3553 (.Swap ⟨1, by decide⟩),
+  [pushAt 3543 2 2112,
+   opAt 3544 .MLOAD,
+   pushAt 3545 0 0,
+   opAt 3546 .MLOAD,
+   opAt 3547 (.Dup ⟨1, by decide⟩),
+   opAt 3548 (.Dup ⟨1, by decide⟩),
+   opAt 3549 .GT,
+   opAt 3550 (.Swap ⟨1, by decide⟩),
+   opAt 3551 .SUB,
+   opAt 3552 (.Dup ⟨2, by decide⟩),
+   opAt 3553 (.Dup ⟨1, by decide⟩),
    opAt 3554 .SUB,
-   opAt 3555 (.Dup ⟨2, by decide⟩),
-   opAt 3556 (.Dup ⟨1, by decide⟩),
-   opAt 3557 .SUB,
-   opAt 3558 (.Swap ⟨2, by decide⟩),
-   opAt 3559 .GT,
-   opAt 3560 .OR,
-   opAt 3561 (.Swap ⟨0, by decide⟩),
-   pushAt 3562 2 1792,
-   opAt 3563 .MSTORE]
+   opAt 3555 (.Swap ⟨2, by decide⟩),
+   opAt 3556 .GT,
+   opAt 3557 .OR,
+   opAt 3558 (.Swap ⟨0, by decide⟩),
+   pushAt 3559 2 1792,
+   opAt 3560 .MSTORE]
 
 def csFixedTail8 : List (Challenge.EvmProof.Stepper.Located Artifact.submissionArtifact .Osaka) :=
-  [opAt 3564 .ISZERO,
-   pushAt 3565 2 2080,
-   opAt 3566 .MLOAD,
-   opAt 3567 .OR,
-   pushAt 3568 2 319,
-   opAt 3569 .NOT,
-   pushAt 3570 2 4747,
-   opAt 3571 .JUMP,
-   opAt 3584 .JUMPDEST,
-   opAt 3585 .MUL,
-   pushAt 3586 2 2112,
-   opAt 3587 .ADD,
-   pushAt 3588 2 2688,
-   opAt 3589 .MLOAD,
-   opAt 3590 (.Swap ⟨1, by decide⟩),
-   opAt 3591 .MCOPY,
-   opAt 3592 .JUMP]
+  [opAt 3561 .ISZERO,
+   pushAt 3562 2 2080,
+   opAt 3563 .MLOAD,
+   opAt 3564 .OR,
+   pushAt 3565 2 319,
+   opAt 3566 .NOT,
+   pushAt 3567 2 4757,
+   opAt 3568 .JUMP,
+   opAt 3581 .JUMPDEST,
+   opAt 3582 .MUL,
+   pushAt 3583 2 2112,
+   opAt 3584 .ADD,
+   pushAt 3585 2 2688,
+   opAt 3586 .MLOAD,
+   opAt 3587 (.Swap ⟨1, by decide⟩),
+   opAt 3588 .MCOPY,
+   opAt 3589 .JUMP]
 
 def csFixedStep4_0 : List (Challenge.EvmProof.Stepper.Located Artifact.submissionArtifact .Osaka) :=
-  [pushAt 3300 2 2208,
-   opAt 3301 .MLOAD,
-   pushAt 3302 1 96,
-   opAt 3303 .MLOAD,
-   opAt 3304 (.Dup ⟨1, by decide⟩),
-   opAt 3305 (.Dup ⟨1, by decide⟩),
-   opAt 3306 .GT,
-   opAt 3307 (.Swap ⟨1, by decide⟩),
-   opAt 3308 .SUB,
-   pushAt 3309 2 1888,
-   opAt 3310 .MSTORE,
-   pushAt 3311 2 4644,
-   opAt 3312 .JUMP]
+  [pushAt 3288 2 2208,
+   opAt 3289 .MLOAD,
+   pushAt 3290 1 96,
+   opAt 3291 .MLOAD,
+   opAt 3292 (.Dup ⟨1, by decide⟩),
+   opAt 3293 (.Dup ⟨1, by decide⟩),
+   opAt 3294 .GT,
+   opAt 3295 (.Swap ⟨1, by decide⟩),
+   opAt 3296 .SUB,
+   pushAt 3297 2 1888,
+   opAt 3298 .MSTORE,
+   pushAt 3299 2 4654,
+   opAt 3300 .JUMP]
 
 def csFixedStep4_1 : List (Challenge.EvmProof.Stepper.Located Artifact.submissionArtifact .Osaka) :=
-  [opAt 3509 .JUMPDEST,
-   pushAt 3510 2 2176,
-   opAt 3511 .MLOAD,
-   pushAt 3512 1 64,
-   opAt 3513 .MLOAD,
-   opAt 3514 (.Dup ⟨1, by decide⟩),
-   opAt 3515 (.Dup ⟨1, by decide⟩),
-   opAt 3516 .GT,
-   opAt 3517 (.Swap ⟨1, by decide⟩),
+  [opAt 3506 .JUMPDEST,
+   pushAt 3507 2 2176,
+   opAt 3508 .MLOAD,
+   pushAt 3509 1 64,
+   opAt 3510 .MLOAD,
+   opAt 3511 (.Dup ⟨1, by decide⟩),
+   opAt 3512 (.Dup ⟨1, by decide⟩),
+   opAt 3513 .GT,
+   opAt 3514 (.Swap ⟨1, by decide⟩),
+   opAt 3515 .SUB,
+   opAt 3516 (.Dup ⟨2, by decide⟩),
+   opAt 3517 (.Dup ⟨1, by decide⟩),
    opAt 3518 .SUB,
-   opAt 3519 (.Dup ⟨2, by decide⟩),
-   opAt 3520 (.Dup ⟨1, by decide⟩),
-   opAt 3521 .SUB,
-   opAt 3522 (.Swap ⟨2, by decide⟩),
-   opAt 3523 .GT,
-   opAt 3524 .OR,
-   opAt 3525 (.Swap ⟨0, by decide⟩),
-   pushAt 3526 2 1856,
-   opAt 3527 .MSTORE]
+   opAt 3519 (.Swap ⟨2, by decide⟩),
+   opAt 3520 .GT,
+   opAt 3521 .OR,
+   opAt 3522 (.Swap ⟨0, by decide⟩),
+   pushAt 3523 2 1856,
+   opAt 3524 .MSTORE]
 
 def csFixedStep4_2 : List (Challenge.EvmProof.Stepper.Located Artifact.submissionArtifact .Osaka) :=
-  [pushAt 3528 2 2144,
-   opAt 3529 .MLOAD,
-   pushAt 3530 1 32,
-   opAt 3531 .MLOAD,
-   opAt 3532 (.Dup ⟨1, by decide⟩),
-   opAt 3533 (.Dup ⟨1, by decide⟩),
-   opAt 3534 .GT,
-   opAt 3535 (.Swap ⟨1, by decide⟩),
+  [pushAt 3525 2 2144,
+   opAt 3526 .MLOAD,
+   pushAt 3527 1 32,
+   opAt 3528 .MLOAD,
+   opAt 3529 (.Dup ⟨1, by decide⟩),
+   opAt 3530 (.Dup ⟨1, by decide⟩),
+   opAt 3531 .GT,
+   opAt 3532 (.Swap ⟨1, by decide⟩),
+   opAt 3533 .SUB,
+   opAt 3534 (.Dup ⟨2, by decide⟩),
+   opAt 3535 (.Dup ⟨1, by decide⟩),
    opAt 3536 .SUB,
-   opAt 3537 (.Dup ⟨2, by decide⟩),
-   opAt 3538 (.Dup ⟨1, by decide⟩),
-   opAt 3539 .SUB,
-   opAt 3540 (.Swap ⟨2, by decide⟩),
-   opAt 3541 .GT,
-   opAt 3542 .OR,
-   opAt 3543 (.Swap ⟨0, by decide⟩),
-   pushAt 3544 2 1824,
-   opAt 3545 .MSTORE]
+   opAt 3537 (.Swap ⟨2, by decide⟩),
+   opAt 3538 .GT,
+   opAt 3539 .OR,
+   opAt 3540 (.Swap ⟨0, by decide⟩),
+   pushAt 3541 2 1824,
+   opAt 3542 .MSTORE]
 
 def csFixedStep4_3 : List (Challenge.EvmProof.Stepper.Located Artifact.submissionArtifact .Osaka) :=
-  [pushAt 3546 2 2112,
-   opAt 3547 .MLOAD,
-   pushAt 3548 0 0,
-   opAt 3549 .MLOAD,
-   opAt 3550 (.Dup ⟨1, by decide⟩),
-   opAt 3551 (.Dup ⟨1, by decide⟩),
-   opAt 3552 .GT,
-   opAt 3553 (.Swap ⟨1, by decide⟩),
+  [pushAt 3543 2 2112,
+   opAt 3544 .MLOAD,
+   pushAt 3545 0 0,
+   opAt 3546 .MLOAD,
+   opAt 3547 (.Dup ⟨1, by decide⟩),
+   opAt 3548 (.Dup ⟨1, by decide⟩),
+   opAt 3549 .GT,
+   opAt 3550 (.Swap ⟨1, by decide⟩),
+   opAt 3551 .SUB,
+   opAt 3552 (.Dup ⟨2, by decide⟩),
+   opAt 3553 (.Dup ⟨1, by decide⟩),
    opAt 3554 .SUB,
-   opAt 3555 (.Dup ⟨2, by decide⟩),
-   opAt 3556 (.Dup ⟨1, by decide⟩),
-   opAt 3557 .SUB,
-   opAt 3558 (.Swap ⟨2, by decide⟩),
-   opAt 3559 .GT,
-   opAt 3560 .OR,
-   opAt 3561 (.Swap ⟨0, by decide⟩),
-   pushAt 3562 2 1792,
-   opAt 3563 .MSTORE]
+   opAt 3555 (.Swap ⟨2, by decide⟩),
+   opAt 3556 .GT,
+   opAt 3557 .OR,
+   opAt 3558 (.Swap ⟨0, by decide⟩),
+   pushAt 3559 2 1792,
+   opAt 3560 .MSTORE]
 
 def csFixedTail4 : List (Challenge.EvmProof.Stepper.Located Artifact.submissionArtifact .Osaka) :=
-  [opAt 3564 .ISZERO,
-   pushAt 3565 2 2080,
-   opAt 3566 .MLOAD,
-   opAt 3567 .OR,
-   pushAt 3568 2 319,
-   opAt 3569 .NOT,
-   pushAt 3570 2 4747,
-   opAt 3571 .JUMP,
-   opAt 3584 .JUMPDEST,
-   opAt 3585 .MUL,
-   pushAt 3586 2 2112,
-   opAt 3587 .ADD,
-   pushAt 3588 2 2688,
-   opAt 3589 .MLOAD,
-   opAt 3590 (.Swap ⟨1, by decide⟩),
-   opAt 3591 .MCOPY,
-   opAt 3592 .JUMP]
+  [opAt 3561 .ISZERO,
+   pushAt 3562 2 2080,
+   opAt 3563 .MLOAD,
+   opAt 3564 .OR,
+   pushAt 3565 2 319,
+   opAt 3566 .NOT,
+   pushAt 3567 2 4757,
+   opAt 3568 .JUMP,
+   opAt 3581 .JUMPDEST,
+   opAt 3582 .MUL,
+   pushAt 3583 2 2112,
+   opAt 3584 .ADD,
+   pushAt 3585 2 2688,
+   opAt 3586 .MLOAD,
+   opAt 3587 (.Swap ⟨1, by decide⟩),
+   opAt 3588 .MCOPY,
+   opAt 3589 .JUMP]
 
-@[simp] theorem fixedPC1618 : Artifact.submissionArtifact.instructionPC 1102 = 1557 := by
+@[simp] theorem fixedPC1618 : Artifact.submissionArtifact.instructionPC 1102 = 1558 := by
   rw [Challenge.Modexp.Submission.Proofs.Bytecode.PCFast.instructionPC_eq_byteLength]
   rfl
 
-@[simp] theorem fixedPC1619 : Artifact.submissionArtifact.instructionPC 1103 = 1560 := by
+@[simp] theorem fixedPC1619 : Artifact.submissionArtifact.instructionPC 1103 = 1561 := by
   rw [Challenge.Modexp.Submission.Proofs.Bytecode.PCFast.instructionPC_eq_byteLength]
   rfl
 
-@[simp] theorem fixedPC3777 : Artifact.submissionArtifact.instructionPC 3400 = 4491 := by
+@[simp] theorem fixedPC3777 : Artifact.submissionArtifact.instructionPC 3397 = 4501 := by
   rw [Challenge.Modexp.Submission.Proofs.Bytecode.PCFast.instructionPC_eq_byteLength]
   rfl
 
-@[simp] theorem fixedJump4975 : Decode.isValidJumpDest Challenge.Modexp.submissionBytecode 4491 = true := by
-  simpa only [Artifact.instructionPC, fixedPC3777] using Artifact.isValidJumpDest_index 3400 (by rfl)
+@[simp] theorem fixedJump4975 : Decode.isValidJumpDest Challenge.Modexp.submissionBytecode 4501 = true := by
+  simpa only [Artifact.instructionPC, fixedPC3777] using Artifact.isValidJumpDest_index 3397 (by rfl)
 
-@[simp] theorem fixedPC3778 : Artifact.submissionArtifact.instructionPC 3401 = 4492 := by
+@[simp] theorem fixedPC3778 : Artifact.submissionArtifact.instructionPC 3398 = 4502 := by
   rw [Challenge.Modexp.Submission.Proofs.Bytecode.PCFast.instructionPC_eq_byteLength]
   rfl
 
-@[simp] theorem fixedPC3779 : Artifact.submissionArtifact.instructionPC 3402 = 4495 := by
+@[simp] theorem fixedPC3779 : Artifact.submissionArtifact.instructionPC 3399 = 4505 := by
   rw [Challenge.Modexp.Submission.Proofs.Bytecode.PCFast.instructionPC_eq_byteLength]
   rfl
 
-@[simp] theorem fixedPC3780 : Artifact.submissionArtifact.instructionPC 3403 = 4496 := by
+@[simp] theorem fixedPC3780 : Artifact.submissionArtifact.instructionPC 3400 = 4506 := by
   rw [Challenge.Modexp.Submission.Proofs.Bytecode.PCFast.instructionPC_eq_byteLength]
   rfl
 
-@[simp] theorem fixedPC3781 : Artifact.submissionArtifact.instructionPC 3404 = 4499 := by
+@[simp] theorem fixedPC3781 : Artifact.submissionArtifact.instructionPC 3401 = 4509 := by
   rw [Challenge.Modexp.Submission.Proofs.Bytecode.PCFast.instructionPC_eq_byteLength]
   rfl
 
-@[simp] theorem fixedPC3782 : Artifact.submissionArtifact.instructionPC 3405 = 4500 := by
+@[simp] theorem fixedPC3782 : Artifact.submissionArtifact.instructionPC 3402 = 4510 := by
   rw [Challenge.Modexp.Submission.Proofs.Bytecode.PCFast.instructionPC_eq_byteLength]
   rfl
 
-@[simp] theorem fixedPC3783 : Artifact.submissionArtifact.instructionPC 3406 = 4503 := by
+@[simp] theorem fixedPC3783 : Artifact.submissionArtifact.instructionPC 3403 = 4513 := by
   rw [Challenge.Modexp.Submission.Proofs.Bytecode.PCFast.instructionPC_eq_byteLength]
   rfl
 
-@[simp] theorem fixedPC3784 : Artifact.submissionArtifact.instructionPC 3407 = 4504 := by
+@[simp] theorem fixedPC3784 : Artifact.submissionArtifact.instructionPC 3404 = 4514 := by
   rw [Challenge.Modexp.Submission.Proofs.Bytecode.PCFast.instructionPC_eq_byteLength]
   rfl
 
-@[simp] theorem fixedPC3785 : Artifact.submissionArtifact.instructionPC 3408 = 4507 := by
+@[simp] theorem fixedPC3785 : Artifact.submissionArtifact.instructionPC 3405 = 4517 := by
   rw [Challenge.Modexp.Submission.Proofs.Bytecode.PCFast.instructionPC_eq_byteLength]
   rfl
 
-@[simp] theorem fixedPC3786 : Artifact.submissionArtifact.instructionPC 3409 = 4508 := by
+@[simp] theorem fixedPC3786 : Artifact.submissionArtifact.instructionPC 3406 = 4518 := by
   rw [Challenge.Modexp.Submission.Proofs.Bytecode.PCFast.instructionPC_eq_byteLength]
   rfl
 
-@[simp] theorem fixedPC3787 : Artifact.submissionArtifact.instructionPC 3410 = 4510 := by
+@[simp] theorem fixedPC3787 : Artifact.submissionArtifact.instructionPC 3407 = 4520 := by
   rw [Challenge.Modexp.Submission.Proofs.Bytecode.PCFast.instructionPC_eq_byteLength]
   rfl
 
-@[simp] theorem fixedPC3788 : Artifact.submissionArtifact.instructionPC 3411 = 4511 := by
+@[simp] theorem fixedPC3788 : Artifact.submissionArtifact.instructionPC 3408 = 4521 := by
   rw [Challenge.Modexp.Submission.Proofs.Bytecode.PCFast.instructionPC_eq_byteLength]
   rfl
 
-@[simp] theorem fixedPC3789 : Artifact.submissionArtifact.instructionPC 3412 = 4514 := by
+@[simp] theorem fixedPC3789 : Artifact.submissionArtifact.instructionPC 3409 = 4524 := by
   rw [Challenge.Modexp.Submission.Proofs.Bytecode.PCFast.instructionPC_eq_byteLength]
   rfl
 
-@[simp] theorem fixedPC3790 : Artifact.submissionArtifact.instructionPC 3413 = 4515 := by
+@[simp] theorem fixedPC3790 : Artifact.submissionArtifact.instructionPC 3410 = 4525 := by
   rw [Challenge.Modexp.Submission.Proofs.Bytecode.PCFast.instructionPC_eq_byteLength]
   rfl
 
-@[simp] theorem fixedPC3791 : Artifact.submissionArtifact.instructionPC 3414 = 4518 := by
+@[simp] theorem fixedPC3791 : Artifact.submissionArtifact.instructionPC 3411 = 4528 := by
   rw [Challenge.Modexp.Submission.Proofs.Bytecode.PCFast.instructionPC_eq_byteLength]
   rfl
 
-@[simp] theorem fixedPC3792 : Artifact.submissionArtifact.instructionPC 3415 = 4519 := by
+@[simp] theorem fixedPC3792 : Artifact.submissionArtifact.instructionPC 3412 = 4529 := by
   rw [Challenge.Modexp.Submission.Proofs.Bytecode.PCFast.instructionPC_eq_byteLength]
   rfl
 
-@[simp] theorem fixedPC3793 : Artifact.submissionArtifact.instructionPC 3416 = 4522 := by
+@[simp] theorem fixedPC3793 : Artifact.submissionArtifact.instructionPC 3413 = 4532 := by
   rw [Challenge.Modexp.Submission.Proofs.Bytecode.PCFast.instructionPC_eq_byteLength]
   rfl
 
-@[simp] theorem fixedPC3794 : Artifact.submissionArtifact.instructionPC 3417 = 4523 := by
+@[simp] theorem fixedPC3794 : Artifact.submissionArtifact.instructionPC 3414 = 4533 := by
   rw [Challenge.Modexp.Submission.Proofs.Bytecode.PCFast.instructionPC_eq_byteLength]
   rfl
 
-@[simp] theorem fixedPC3795 : Artifact.submissionArtifact.instructionPC 3418 = 4524 := by
+@[simp] theorem fixedPC3795 : Artifact.submissionArtifact.instructionPC 3415 = 4534 := by
   rw [Challenge.Modexp.Submission.Proofs.Bytecode.PCFast.instructionPC_eq_byteLength]
   rfl
 
-@[simp] theorem fixedPC3796 : Artifact.submissionArtifact.instructionPC 3419 = 4527 := by
+@[simp] theorem fixedPC3796 : Artifact.submissionArtifact.instructionPC 3416 = 4537 := by
   rw [Challenge.Modexp.Submission.Proofs.Bytecode.PCFast.instructionPC_eq_byteLength]
   rfl
 
-@[simp] theorem fixedPC3797 : Artifact.submissionArtifact.instructionPC 3420 = 4528 := by
+@[simp] theorem fixedPC3797 : Artifact.submissionArtifact.instructionPC 3417 = 4538 := by
   rw [Challenge.Modexp.Submission.Proofs.Bytecode.PCFast.instructionPC_eq_byteLength]
   rfl
 
-@[simp] theorem fixedPC3798 : Artifact.submissionArtifact.instructionPC 3420 = 4528 := fixedPC3797
+@[simp] theorem fixedPC3798 : Artifact.submissionArtifact.instructionPC 3417 = 4538 := fixedPC3797
 
-@[simp] theorem fixedPC3799 : Artifact.submissionArtifact.instructionPC 3420 = 4528 := fixedPC3797
+@[simp] theorem fixedPC3799 : Artifact.submissionArtifact.instructionPC 3417 = 4538 := fixedPC3797
 
-@[simp] theorem fixedPC3800 : Artifact.submissionArtifact.instructionPC 3421 = 4529 := by
+@[simp] theorem fixedPC3800 : Artifact.submissionArtifact.instructionPC 3418 = 4539 := by
   rw [Challenge.Modexp.Submission.Proofs.Bytecode.PCFast.instructionPC_eq_byteLength]
   rfl
 
-@[simp] theorem fixedPC3801 : Artifact.submissionArtifact.instructionPC 3422 = 4530 := by
+@[simp] theorem fixedPC3801 : Artifact.submissionArtifact.instructionPC 3419 = 4540 := by
   rw [Challenge.Modexp.Submission.Proofs.Bytecode.PCFast.instructionPC_eq_byteLength]
   rfl
 
-@[simp] theorem fixedPC3802 : Artifact.submissionArtifact.instructionPC 3423 = 4531 := by
+@[simp] theorem fixedPC3802 : Artifact.submissionArtifact.instructionPC 3420 = 4541 := by
   rw [Challenge.Modexp.Submission.Proofs.Bytecode.PCFast.instructionPC_eq_byteLength]
   rfl
 
-@[simp] theorem fixedPC3803 : Artifact.submissionArtifact.instructionPC 3424 = 4534 := by
+@[simp] theorem fixedPC3803 : Artifact.submissionArtifact.instructionPC 3421 = 4544 := by
   rw [Challenge.Modexp.Submission.Proofs.Bytecode.PCFast.instructionPC_eq_byteLength]
   rfl
 
-@[simp] theorem fixedPC3804 : Artifact.submissionArtifact.instructionPC 3425 = 4535 := by
+@[simp] theorem fixedPC3804 : Artifact.submissionArtifact.instructionPC 3422 = 4545 := by
   rw [Challenge.Modexp.Submission.Proofs.Bytecode.PCFast.instructionPC_eq_byteLength]
   rfl
 
-@[simp] theorem fixedJump5023 : Decode.isValidJumpDest Challenge.Modexp.submissionBytecode 4535 = true := by
-  simpa only [Artifact.instructionPC, fixedPC3804] using Artifact.isValidJumpDest_index 3425 (by rfl)
+@[simp] theorem fixedJump5023 : Decode.isValidJumpDest Challenge.Modexp.submissionBytecode 4545 = true := by
+  simpa only [Artifact.instructionPC, fixedPC3804] using Artifact.isValidJumpDest_index 3422 (by rfl)
 
-@[simp] theorem fixedPC3805 : Artifact.submissionArtifact.instructionPC 3426 = 4536 := by
+@[simp] theorem fixedPC3805 : Artifact.submissionArtifact.instructionPC 3423 = 4546 := by
   rw [Challenge.Modexp.Submission.Proofs.Bytecode.PCFast.instructionPC_eq_byteLength]
   rfl
 
-@[simp] theorem fixedPC3806 : Artifact.submissionArtifact.instructionPC 3427 = 4539 := by
+@[simp] theorem fixedPC3806 : Artifact.submissionArtifact.instructionPC 3424 = 4549 := by
   rw [Challenge.Modexp.Submission.Proofs.Bytecode.PCFast.instructionPC_eq_byteLength]
   rfl
 
-@[simp] theorem fixedPC3807 : Artifact.submissionArtifact.instructionPC 3428 = 4540 := by
+@[simp] theorem fixedPC3807 : Artifact.submissionArtifact.instructionPC 3425 = 4550 := by
   rw [Challenge.Modexp.Submission.Proofs.Bytecode.PCFast.instructionPC_eq_byteLength]
   rfl
 
-@[simp] theorem fixedPC3808 : Artifact.submissionArtifact.instructionPC 3429 = 4542 := by
+@[simp] theorem fixedPC3808 : Artifact.submissionArtifact.instructionPC 3426 = 4552 := by
   rw [Challenge.Modexp.Submission.Proofs.Bytecode.PCFast.instructionPC_eq_byteLength]
   rfl
 
-@[simp] theorem fixedPC3809 : Artifact.submissionArtifact.instructionPC 3430 = 4543 := by
+@[simp] theorem fixedPC3809 : Artifact.submissionArtifact.instructionPC 3427 = 4553 := by
   rw [Challenge.Modexp.Submission.Proofs.Bytecode.PCFast.instructionPC_eq_byteLength]
   rfl
 
-@[simp] theorem fixedPC3810 : Artifact.submissionArtifact.instructionPC 3431 = 4544 := by
+@[simp] theorem fixedPC3810 : Artifact.submissionArtifact.instructionPC 3428 = 4554 := by
   rw [Challenge.Modexp.Submission.Proofs.Bytecode.PCFast.instructionPC_eq_byteLength]
   rfl
 
-@[simp] theorem fixedPC3811 : Artifact.submissionArtifact.instructionPC 3432 = 4545 := by
+@[simp] theorem fixedPC3811 : Artifact.submissionArtifact.instructionPC 3429 = 4555 := by
   rw [Challenge.Modexp.Submission.Proofs.Bytecode.PCFast.instructionPC_eq_byteLength]
   rfl
 
-@[simp] theorem fixedPC3812 : Artifact.submissionArtifact.instructionPC 3433 = 4546 := by
+@[simp] theorem fixedPC3812 : Artifact.submissionArtifact.instructionPC 3430 = 4556 := by
   rw [Challenge.Modexp.Submission.Proofs.Bytecode.PCFast.instructionPC_eq_byteLength]
   rfl
 
-@[simp] theorem fixedPC3813 : Artifact.submissionArtifact.instructionPC 3434 = 4547 := by
+@[simp] theorem fixedPC3813 : Artifact.submissionArtifact.instructionPC 3431 = 4557 := by
   rw [Challenge.Modexp.Submission.Proofs.Bytecode.PCFast.instructionPC_eq_byteLength]
   rfl
 
-@[simp] theorem fixedPC3814 : Artifact.submissionArtifact.instructionPC 3435 = 4548 := by
+@[simp] theorem fixedPC3814 : Artifact.submissionArtifact.instructionPC 3432 = 4558 := by
   rw [Challenge.Modexp.Submission.Proofs.Bytecode.PCFast.instructionPC_eq_byteLength]
   rfl
 
-@[simp] theorem fixedPC3815 : Artifact.submissionArtifact.instructionPC 3436 = 4551 := by
+@[simp] theorem fixedPC3815 : Artifact.submissionArtifact.instructionPC 3433 = 4561 := by
   rw [Challenge.Modexp.Submission.Proofs.Bytecode.PCFast.instructionPC_eq_byteLength]
   rfl
 
-@[simp] theorem fixedPC3816 : Artifact.submissionArtifact.instructionPC 3437 = 4552 := by
+@[simp] theorem fixedPC3816 : Artifact.submissionArtifact.instructionPC 3434 = 4562 := by
   rw [Challenge.Modexp.Submission.Proofs.Bytecode.PCFast.instructionPC_eq_byteLength]
   rfl
 
-@[simp] theorem fixedPC3817 : Artifact.submissionArtifact.instructionPC 3438 = 4555 := by
+@[simp] theorem fixedPC3817 : Artifact.submissionArtifact.instructionPC 3435 = 4565 := by
   rw [Challenge.Modexp.Submission.Proofs.Bytecode.PCFast.instructionPC_eq_byteLength]
   rfl
 
-@[simp] theorem fixedPC3818 : Artifact.submissionArtifact.instructionPC 3439 = 4556 := by
+@[simp] theorem fixedPC3818 : Artifact.submissionArtifact.instructionPC 3436 = 4566 := by
   rw [Challenge.Modexp.Submission.Proofs.Bytecode.PCFast.instructionPC_eq_byteLength]
   rfl
 
-@[simp] theorem fixedPC3819 : Artifact.submissionArtifact.instructionPC 3440 = 4558 := by
+@[simp] theorem fixedPC3819 : Artifact.submissionArtifact.instructionPC 3437 = 4568 := by
   rw [Challenge.Modexp.Submission.Proofs.Bytecode.PCFast.instructionPC_eq_byteLength]
   rfl
 
-@[simp] theorem fixedPC3820 : Artifact.submissionArtifact.instructionPC 3441 = 4559 := by
+@[simp] theorem fixedPC3820 : Artifact.submissionArtifact.instructionPC 3438 = 4569 := by
   rw [Challenge.Modexp.Submission.Proofs.Bytecode.PCFast.instructionPC_eq_byteLength]
   rfl
 
-@[simp] theorem fixedPC3821 : Artifact.submissionArtifact.instructionPC 3442 = 4560 := by
+@[simp] theorem fixedPC3821 : Artifact.submissionArtifact.instructionPC 3439 = 4570 := by
   rw [Challenge.Modexp.Submission.Proofs.Bytecode.PCFast.instructionPC_eq_byteLength]
   rfl
 
-@[simp] theorem fixedPC3822 : Artifact.submissionArtifact.instructionPC 3443 = 4561 := by
+@[simp] theorem fixedPC3822 : Artifact.submissionArtifact.instructionPC 3440 = 4571 := by
   rw [Challenge.Modexp.Submission.Proofs.Bytecode.PCFast.instructionPC_eq_byteLength]
   rfl
 
-@[simp] theorem fixedPC3823 : Artifact.submissionArtifact.instructionPC 3444 = 4562 := by
+@[simp] theorem fixedPC3823 : Artifact.submissionArtifact.instructionPC 3441 = 4572 := by
   rw [Challenge.Modexp.Submission.Proofs.Bytecode.PCFast.instructionPC_eq_byteLength]
   rfl
 
-@[simp] theorem fixedPC3824 : Artifact.submissionArtifact.instructionPC 3445 = 4563 := by
+@[simp] theorem fixedPC3824 : Artifact.submissionArtifact.instructionPC 3442 = 4573 := by
   rw [Challenge.Modexp.Submission.Proofs.Bytecode.PCFast.instructionPC_eq_byteLength]
   rfl
 
-@[simp] theorem fixedPC3825 : Artifact.submissionArtifact.instructionPC 3446 = 4564 := by
+@[simp] theorem fixedPC3825 : Artifact.submissionArtifact.instructionPC 3443 = 4574 := by
   rw [Challenge.Modexp.Submission.Proofs.Bytecode.PCFast.instructionPC_eq_byteLength]
   rfl
 
-@[simp] theorem fixedPC3826 : Artifact.submissionArtifact.instructionPC 3447 = 4565 := by
+@[simp] theorem fixedPC3826 : Artifact.submissionArtifact.instructionPC 3444 = 4575 := by
   rw [Challenge.Modexp.Submission.Proofs.Bytecode.PCFast.instructionPC_eq_byteLength]
   rfl
 
-@[simp] theorem fixedPC3827 : Artifact.submissionArtifact.instructionPC 3448 = 4566 := by
+@[simp] theorem fixedPC3827 : Artifact.submissionArtifact.instructionPC 3445 = 4576 := by
   rw [Challenge.Modexp.Submission.Proofs.Bytecode.PCFast.instructionPC_eq_byteLength]
   rfl
 
-@[simp] theorem fixedPC3828 : Artifact.submissionArtifact.instructionPC 3449 = 4567 := by
+@[simp] theorem fixedPC3828 : Artifact.submissionArtifact.instructionPC 3446 = 4577 := by
   rw [Challenge.Modexp.Submission.Proofs.Bytecode.PCFast.instructionPC_eq_byteLength]
   rfl
 
-@[simp] theorem fixedPC3829 : Artifact.submissionArtifact.instructionPC 3450 = 4568 := by
+@[simp] theorem fixedPC3829 : Artifact.submissionArtifact.instructionPC 3447 = 4578 := by
   rw [Challenge.Modexp.Submission.Proofs.Bytecode.PCFast.instructionPC_eq_byteLength]
   rfl
 
-@[simp] theorem fixedPC3830 : Artifact.submissionArtifact.instructionPC 3451 = 4569 := by
+@[simp] theorem fixedPC3830 : Artifact.submissionArtifact.instructionPC 3448 = 4579 := by
   rw [Challenge.Modexp.Submission.Proofs.Bytecode.PCFast.instructionPC_eq_byteLength]
   rfl
 
-@[simp] theorem fixedPC3831 : Artifact.submissionArtifact.instructionPC 3452 = 4570 := by
+@[simp] theorem fixedPC3831 : Artifact.submissionArtifact.instructionPC 3449 = 4580 := by
   rw [Challenge.Modexp.Submission.Proofs.Bytecode.PCFast.instructionPC_eq_byteLength]
   rfl
 
-@[simp] theorem fixedPC3832 : Artifact.submissionArtifact.instructionPC 3453 = 4571 := by
+@[simp] theorem fixedPC3832 : Artifact.submissionArtifact.instructionPC 3450 = 4581 := by
   rw [Challenge.Modexp.Submission.Proofs.Bytecode.PCFast.instructionPC_eq_byteLength]
   rfl
 
-@[simp] theorem fixedPC3833 : Artifact.submissionArtifact.instructionPC 3454 = 4574 := by
+@[simp] theorem fixedPC3833 : Artifact.submissionArtifact.instructionPC 3451 = 4584 := by
   rw [Challenge.Modexp.Submission.Proofs.Bytecode.PCFast.instructionPC_eq_byteLength]
   rfl
 
-@[simp] theorem fixedPC3834 : Artifact.submissionArtifact.instructionPC 3455 = 4575 := by
+@[simp] theorem fixedPC3834 : Artifact.submissionArtifact.instructionPC 3452 = 4585 := by
   rw [Challenge.Modexp.Submission.Proofs.Bytecode.PCFast.instructionPC_eq_byteLength]
   rfl
 
-@[simp] theorem fixedPC3835 : Artifact.submissionArtifact.instructionPC 3456 = 4578 := by
+@[simp] theorem fixedPC3835 : Artifact.submissionArtifact.instructionPC 3453 = 4588 := by
   rw [Challenge.Modexp.Submission.Proofs.Bytecode.PCFast.instructionPC_eq_byteLength]
   rfl
 
-@[simp] theorem fixedPC3836 : Artifact.submissionArtifact.instructionPC 3457 = 4579 := by
+@[simp] theorem fixedPC3836 : Artifact.submissionArtifact.instructionPC 3454 = 4589 := by
   rw [Challenge.Modexp.Submission.Proofs.Bytecode.PCFast.instructionPC_eq_byteLength]
   rfl
 
-@[simp] theorem fixedPC3837 : Artifact.submissionArtifact.instructionPC 3458 = 4581 := by
+@[simp] theorem fixedPC3837 : Artifact.submissionArtifact.instructionPC 3455 = 4591 := by
   rw [Challenge.Modexp.Submission.Proofs.Bytecode.PCFast.instructionPC_eq_byteLength]
   rfl
 
-@[simp] theorem fixedPC3838 : Artifact.submissionArtifact.instructionPC 3459 = 4582 := by
+@[simp] theorem fixedPC3838 : Artifact.submissionArtifact.instructionPC 3456 = 4592 := by
   rw [Challenge.Modexp.Submission.Proofs.Bytecode.PCFast.instructionPC_eq_byteLength]
   rfl
 
-@[simp] theorem fixedPC3839 : Artifact.submissionArtifact.instructionPC 3460 = 4583 := by
+@[simp] theorem fixedPC3839 : Artifact.submissionArtifact.instructionPC 3457 = 4593 := by
   rw [Challenge.Modexp.Submission.Proofs.Bytecode.PCFast.instructionPC_eq_byteLength]
   rfl
 
-@[simp] theorem fixedPC3840 : Artifact.submissionArtifact.instructionPC 3461 = 4584 := by
+@[simp] theorem fixedPC3840 : Artifact.submissionArtifact.instructionPC 3458 = 4594 := by
   rw [Challenge.Modexp.Submission.Proofs.Bytecode.PCFast.instructionPC_eq_byteLength]
   rfl
 
-@[simp] theorem fixedPC3841 : Artifact.submissionArtifact.instructionPC 3462 = 4585 := by
+@[simp] theorem fixedPC3841 : Artifact.submissionArtifact.instructionPC 3459 = 4595 := by
   rw [Challenge.Modexp.Submission.Proofs.Bytecode.PCFast.instructionPC_eq_byteLength]
   rfl
 
-@[simp] theorem fixedPC3842 : Artifact.submissionArtifact.instructionPC 3463 = 4586 := by
+@[simp] theorem fixedPC3842 : Artifact.submissionArtifact.instructionPC 3460 = 4596 := by
   rw [Challenge.Modexp.Submission.Proofs.Bytecode.PCFast.instructionPC_eq_byteLength]
   rfl
 
-@[simp] theorem fixedPC3843 : Artifact.submissionArtifact.instructionPC 3464 = 4587 := by
+@[simp] theorem fixedPC3843 : Artifact.submissionArtifact.instructionPC 3461 = 4597 := by
   rw [Challenge.Modexp.Submission.Proofs.Bytecode.PCFast.instructionPC_eq_byteLength]
   rfl
 
-@[simp] theorem fixedPC3844 : Artifact.submissionArtifact.instructionPC 3465 = 4588 := by
+@[simp] theorem fixedPC3844 : Artifact.submissionArtifact.instructionPC 3462 = 4598 := by
   rw [Challenge.Modexp.Submission.Proofs.Bytecode.PCFast.instructionPC_eq_byteLength]
   rfl
 
-@[simp] theorem fixedPC3845 : Artifact.submissionArtifact.instructionPC 3466 = 4589 := by
+@[simp] theorem fixedPC3845 : Artifact.submissionArtifact.instructionPC 3463 = 4599 := by
   rw [Challenge.Modexp.Submission.Proofs.Bytecode.PCFast.instructionPC_eq_byteLength]
   rfl
 
-@[simp] theorem fixedPC3846 : Artifact.submissionArtifact.instructionPC 3467 = 4590 := by
+@[simp] theorem fixedPC3846 : Artifact.submissionArtifact.instructionPC 3464 = 4600 := by
   rw [Challenge.Modexp.Submission.Proofs.Bytecode.PCFast.instructionPC_eq_byteLength]
   rfl
 
-@[simp] theorem fixedPC3847 : Artifact.submissionArtifact.instructionPC 3468 = 4591 := by
+@[simp] theorem fixedPC3847 : Artifact.submissionArtifact.instructionPC 3465 = 4601 := by
   rw [Challenge.Modexp.Submission.Proofs.Bytecode.PCFast.instructionPC_eq_byteLength]
   rfl
 
-@[simp] theorem fixedPC3848 : Artifact.submissionArtifact.instructionPC 3469 = 4592 := by
+@[simp] theorem fixedPC3848 : Artifact.submissionArtifact.instructionPC 3466 = 4602 := by
   rw [Challenge.Modexp.Submission.Proofs.Bytecode.PCFast.instructionPC_eq_byteLength]
   rfl
 
-@[simp] theorem fixedPC3849 : Artifact.submissionArtifact.instructionPC 3470 = 4593 := by
+@[simp] theorem fixedPC3849 : Artifact.submissionArtifact.instructionPC 3467 = 4603 := by
   rw [Challenge.Modexp.Submission.Proofs.Bytecode.PCFast.instructionPC_eq_byteLength]
   rfl
 
-@[simp] theorem fixedPC3850 : Artifact.submissionArtifact.instructionPC 3471 = 4594 := by
+@[simp] theorem fixedPC3850 : Artifact.submissionArtifact.instructionPC 3468 = 4604 := by
   rw [Challenge.Modexp.Submission.Proofs.Bytecode.PCFast.instructionPC_eq_byteLength]
   rfl
 
-@[simp] theorem fixedPC3851 : Artifact.submissionArtifact.instructionPC 3472 = 4597 := by
+@[simp] theorem fixedPC3851 : Artifact.submissionArtifact.instructionPC 3469 = 4607 := by
   rw [Challenge.Modexp.Submission.Proofs.Bytecode.PCFast.instructionPC_eq_byteLength]
   rfl
 
-@[simp] theorem fixedPC3852 : Artifact.submissionArtifact.instructionPC 3473 = 4598 := by
+@[simp] theorem fixedPC3852 : Artifact.submissionArtifact.instructionPC 3470 = 4608 := by
   rw [Challenge.Modexp.Submission.Proofs.Bytecode.PCFast.instructionPC_eq_byteLength]
   rfl
 
-@[simp] theorem fixedPC3853 : Artifact.submissionArtifact.instructionPC 3474 = 4601 := by
+@[simp] theorem fixedPC3853 : Artifact.submissionArtifact.instructionPC 3471 = 4611 := by
   rw [Challenge.Modexp.Submission.Proofs.Bytecode.PCFast.instructionPC_eq_byteLength]
   rfl
 
-@[simp] theorem fixedPC3854 : Artifact.submissionArtifact.instructionPC 3475 = 4602 := by
+@[simp] theorem fixedPC3854 : Artifact.submissionArtifact.instructionPC 3472 = 4612 := by
   rw [Challenge.Modexp.Submission.Proofs.Bytecode.PCFast.instructionPC_eq_byteLength]
   rfl
 
-@[simp] theorem fixedPC3855 : Artifact.submissionArtifact.instructionPC 3476 = 4604 := by
+@[simp] theorem fixedPC3855 : Artifact.submissionArtifact.instructionPC 3473 = 4614 := by
   rw [Challenge.Modexp.Submission.Proofs.Bytecode.PCFast.instructionPC_eq_byteLength]
   rfl
 
-@[simp] theorem fixedPC3856 : Artifact.submissionArtifact.instructionPC 3477 = 4605 := by
+@[simp] theorem fixedPC3856 : Artifact.submissionArtifact.instructionPC 3474 = 4615 := by
   rw [Challenge.Modexp.Submission.Proofs.Bytecode.PCFast.instructionPC_eq_byteLength]
   rfl
 
-@[simp] theorem fixedPC3857 : Artifact.submissionArtifact.instructionPC 3478 = 4606 := by
+@[simp] theorem fixedPC3857 : Artifact.submissionArtifact.instructionPC 3475 = 4616 := by
   rw [Challenge.Modexp.Submission.Proofs.Bytecode.PCFast.instructionPC_eq_byteLength]
   rfl
 
-@[simp] theorem fixedPC3858 : Artifact.submissionArtifact.instructionPC 3479 = 4607 := by
+@[simp] theorem fixedPC3858 : Artifact.submissionArtifact.instructionPC 3476 = 4617 := by
   rw [Challenge.Modexp.Submission.Proofs.Bytecode.PCFast.instructionPC_eq_byteLength]
   rfl
 
-@[simp] theorem fixedPC3859 : Artifact.submissionArtifact.instructionPC 3480 = 4608 := by
+@[simp] theorem fixedPC3859 : Artifact.submissionArtifact.instructionPC 3477 = 4618 := by
   rw [Challenge.Modexp.Submission.Proofs.Bytecode.PCFast.instructionPC_eq_byteLength]
   rfl
 
-@[simp] theorem fixedPC3860 : Artifact.submissionArtifact.instructionPC 3481 = 4609 := by
+@[simp] theorem fixedPC3860 : Artifact.submissionArtifact.instructionPC 3478 = 4619 := by
   rw [Challenge.Modexp.Submission.Proofs.Bytecode.PCFast.instructionPC_eq_byteLength]
   rfl
 
-@[simp] theorem fixedPC3861 : Artifact.submissionArtifact.instructionPC 3482 = 4610 := by
+@[simp] theorem fixedPC3861 : Artifact.submissionArtifact.instructionPC 3479 = 4620 := by
   rw [Challenge.Modexp.Submission.Proofs.Bytecode.PCFast.instructionPC_eq_byteLength]
   rfl
 
-@[simp] theorem fixedPC3862 : Artifact.submissionArtifact.instructionPC 3483 = 4611 := by
+@[simp] theorem fixedPC3862 : Artifact.submissionArtifact.instructionPC 3480 = 4621 := by
   rw [Challenge.Modexp.Submission.Proofs.Bytecode.PCFast.instructionPC_eq_byteLength]
   rfl
 
-@[simp] theorem fixedPC3863 : Artifact.submissionArtifact.instructionPC 3484 = 4612 := by
+@[simp] theorem fixedPC3863 : Artifact.submissionArtifact.instructionPC 3481 = 4622 := by
   rw [Challenge.Modexp.Submission.Proofs.Bytecode.PCFast.instructionPC_eq_byteLength]
   rfl
 
-@[simp] theorem fixedPC3864 : Artifact.submissionArtifact.instructionPC 3485 = 4613 := by
+@[simp] theorem fixedPC3864 : Artifact.submissionArtifact.instructionPC 3482 = 4623 := by
   rw [Challenge.Modexp.Submission.Proofs.Bytecode.PCFast.instructionPC_eq_byteLength]
   rfl
 
-@[simp] theorem fixedPC3865 : Artifact.submissionArtifact.instructionPC 3486 = 4614 := by
+@[simp] theorem fixedPC3865 : Artifact.submissionArtifact.instructionPC 3483 = 4624 := by
   rw [Challenge.Modexp.Submission.Proofs.Bytecode.PCFast.instructionPC_eq_byteLength]
   rfl
 
-@[simp] theorem fixedPC3866 : Artifact.submissionArtifact.instructionPC 3487 = 4615 := by
+@[simp] theorem fixedPC3866 : Artifact.submissionArtifact.instructionPC 3484 = 4625 := by
   rw [Challenge.Modexp.Submission.Proofs.Bytecode.PCFast.instructionPC_eq_byteLength]
   rfl
 
-@[simp] theorem fixedPC3867 : Artifact.submissionArtifact.instructionPC 3488 = 4616 := by
+@[simp] theorem fixedPC3867 : Artifact.submissionArtifact.instructionPC 3485 = 4626 := by
   rw [Challenge.Modexp.Submission.Proofs.Bytecode.PCFast.instructionPC_eq_byteLength]
   rfl
 
-@[simp] theorem fixedPC3868 : Artifact.submissionArtifact.instructionPC 3489 = 4617 := by
+@[simp] theorem fixedPC3868 : Artifact.submissionArtifact.instructionPC 3486 = 4627 := by
   rw [Challenge.Modexp.Submission.Proofs.Bytecode.PCFast.instructionPC_eq_byteLength]
   rfl
 
-@[simp] theorem fixedPC3869 : Artifact.submissionArtifact.instructionPC 3490 = 4620 := by
+@[simp] theorem fixedPC3869 : Artifact.submissionArtifact.instructionPC 3487 = 4630 := by
   rw [Challenge.Modexp.Submission.Proofs.Bytecode.PCFast.instructionPC_eq_byteLength]
   rfl
 
-@[simp] theorem fixedPC3871 : Artifact.submissionArtifact.instructionPC 3491 = 4621 := by
+@[simp] theorem fixedPC3871 : Artifact.submissionArtifact.instructionPC 3488 = 4631 := by
   rw [Challenge.Modexp.Submission.Proofs.Bytecode.PCFast.instructionPC_eq_byteLength]
   rfl
 
-@[simp] theorem fixedPC3872 : Artifact.submissionArtifact.instructionPC 3492 = 4624 := by
+@[simp] theorem fixedPC3872 : Artifact.submissionArtifact.instructionPC 3489 = 4634 := by
   rw [Challenge.Modexp.Submission.Proofs.Bytecode.PCFast.instructionPC_eq_byteLength]
   rfl
 
-@[simp] theorem fixedPC3873 : Artifact.submissionArtifact.instructionPC 3493 = 4625 := by
+@[simp] theorem fixedPC3873 : Artifact.submissionArtifact.instructionPC 3490 = 4635 := by
   rw [Challenge.Modexp.Submission.Proofs.Bytecode.PCFast.instructionPC_eq_byteLength]
   rfl
 
-@[simp] theorem fixedPC3874 : Artifact.submissionArtifact.instructionPC 3494 = 4627 := by
+@[simp] theorem fixedPC3874 : Artifact.submissionArtifact.instructionPC 3491 = 4637 := by
   rw [Challenge.Modexp.Submission.Proofs.Bytecode.PCFast.instructionPC_eq_byteLength]
   rfl
 
-@[simp] theorem fixedPC3875 : Artifact.submissionArtifact.instructionPC 3495 = 4628 := by
+@[simp] theorem fixedPC3875 : Artifact.submissionArtifact.instructionPC 3492 = 4638 := by
   rw [Challenge.Modexp.Submission.Proofs.Bytecode.PCFast.instructionPC_eq_byteLength]
   rfl
 
-@[simp] theorem fixedPC3876 : Artifact.submissionArtifact.instructionPC 3496 = 4629 := by
+@[simp] theorem fixedPC3876 : Artifact.submissionArtifact.instructionPC 3493 = 4639 := by
   rw [Challenge.Modexp.Submission.Proofs.Bytecode.PCFast.instructionPC_eq_byteLength]
   rfl
 
-@[simp] theorem fixedPC3877 : Artifact.submissionArtifact.instructionPC 3497 = 4630 := by
+@[simp] theorem fixedPC3877 : Artifact.submissionArtifact.instructionPC 3494 = 4640 := by
   rw [Challenge.Modexp.Submission.Proofs.Bytecode.PCFast.instructionPC_eq_byteLength]
   rfl
 
-@[simp] theorem fixedPC3878 : Artifact.submissionArtifact.instructionPC 3498 = 4631 := by
+@[simp] theorem fixedPC3878 : Artifact.submissionArtifact.instructionPC 3495 = 4641 := by
   rw [Challenge.Modexp.Submission.Proofs.Bytecode.PCFast.instructionPC_eq_byteLength]
   rfl
 
-@[simp] theorem fixedPC3879 : Artifact.submissionArtifact.instructionPC 3499 = 4632 := by
+@[simp] theorem fixedPC3879 : Artifact.submissionArtifact.instructionPC 3496 = 4642 := by
   rw [Challenge.Modexp.Submission.Proofs.Bytecode.PCFast.instructionPC_eq_byteLength]
   rfl
 
-@[simp] theorem fixedPC3880 : Artifact.submissionArtifact.instructionPC 3500 = 4633 := by
+@[simp] theorem fixedPC3880 : Artifact.submissionArtifact.instructionPC 3497 = 4643 := by
   rw [Challenge.Modexp.Submission.Proofs.Bytecode.PCFast.instructionPC_eq_byteLength]
   rfl
 
-@[simp] theorem fixedPC3881 : Artifact.submissionArtifact.instructionPC 3501 = 4634 := by
+@[simp] theorem fixedPC3881 : Artifact.submissionArtifact.instructionPC 3498 = 4644 := by
   rw [Challenge.Modexp.Submission.Proofs.Bytecode.PCFast.instructionPC_eq_byteLength]
   rfl
 
-@[simp] theorem fixedPC3882 : Artifact.submissionArtifact.instructionPC 3502 = 4635 := by
+@[simp] theorem fixedPC3882 : Artifact.submissionArtifact.instructionPC 3499 = 4645 := by
   rw [Challenge.Modexp.Submission.Proofs.Bytecode.PCFast.instructionPC_eq_byteLength]
   rfl
 
-@[simp] theorem fixedPC3883 : Artifact.submissionArtifact.instructionPC 3503 = 4636 := by
+@[simp] theorem fixedPC3883 : Artifact.submissionArtifact.instructionPC 3500 = 4646 := by
   rw [Challenge.Modexp.Submission.Proofs.Bytecode.PCFast.instructionPC_eq_byteLength]
   rfl
 
-@[simp] theorem fixedPC3884 : Artifact.submissionArtifact.instructionPC 3504 = 4637 := by
+@[simp] theorem fixedPC3884 : Artifact.submissionArtifact.instructionPC 3501 = 4647 := by
   rw [Challenge.Modexp.Submission.Proofs.Bytecode.PCFast.instructionPC_eq_byteLength]
   rfl
 
-@[simp] theorem fixedPC3885 : Artifact.submissionArtifact.instructionPC 3505 = 4638 := by
+@[simp] theorem fixedPC3885 : Artifact.submissionArtifact.instructionPC 3502 = 4648 := by
   rw [Challenge.Modexp.Submission.Proofs.Bytecode.PCFast.instructionPC_eq_byteLength]
   rfl
 
-@[simp] theorem fixedPC3886 : Artifact.submissionArtifact.instructionPC 3506 = 4639 := by
+@[simp] theorem fixedPC3886 : Artifact.submissionArtifact.instructionPC 3503 = 4649 := by
   rw [Challenge.Modexp.Submission.Proofs.Bytecode.PCFast.instructionPC_eq_byteLength]
   rfl
 
-@[simp] theorem fixedPC3887 : Artifact.submissionArtifact.instructionPC 3507 = 4640 := by
+@[simp] theorem fixedPC3887 : Artifact.submissionArtifact.instructionPC 3504 = 4650 := by
   rw [Challenge.Modexp.Submission.Proofs.Bytecode.PCFast.instructionPC_eq_byteLength]
   rfl
 
-@[simp] theorem fixedPC3888 : Artifact.submissionArtifact.instructionPC 3508 = 4643 := by
+@[simp] theorem fixedPC3888 : Artifact.submissionArtifact.instructionPC 3505 = 4653 := by
   rw [Challenge.Modexp.Submission.Proofs.Bytecode.PCFast.instructionPC_eq_byteLength]
   rfl
 
-@[simp] theorem fixedPC3889 : Artifact.submissionArtifact.instructionPC 3509 = 4644 := by
+@[simp] theorem fixedPC3889 : Artifact.submissionArtifact.instructionPC 3506 = 4654 := by
   rw [Challenge.Modexp.Submission.Proofs.Bytecode.PCFast.instructionPC_eq_byteLength]
   rfl
 
-@[simp] theorem fixedJump5133 : Decode.isValidJumpDest Challenge.Modexp.submissionBytecode 4644 = true := by
-  simpa only [Artifact.instructionPC, fixedPC3889] using Artifact.isValidJumpDest_index 3509 (by rfl)
+@[simp] theorem fixedJump5133 : Decode.isValidJumpDest Challenge.Modexp.submissionBytecode 4654 = true := by
+  simpa only [Artifact.instructionPC, fixedPC3889] using Artifact.isValidJumpDest_index 3506 (by rfl)
 
-@[simp] theorem fixedPC3890 : Artifact.submissionArtifact.instructionPC 3510 = 4645 := by
+@[simp] theorem fixedPC3890 : Artifact.submissionArtifact.instructionPC 3507 = 4655 := by
   rw [Challenge.Modexp.Submission.Proofs.Bytecode.PCFast.instructionPC_eq_byteLength]
   rfl
 
-@[simp] theorem fixedPC3891 : Artifact.submissionArtifact.instructionPC 3511 = 4648 := by
+@[simp] theorem fixedPC3891 : Artifact.submissionArtifact.instructionPC 3508 = 4658 := by
   rw [Challenge.Modexp.Submission.Proofs.Bytecode.PCFast.instructionPC_eq_byteLength]
   rfl
 
-@[simp] theorem fixedPC3892 : Artifact.submissionArtifact.instructionPC 3512 = 4649 := by
+@[simp] theorem fixedPC3892 : Artifact.submissionArtifact.instructionPC 3509 = 4659 := by
   rw [Challenge.Modexp.Submission.Proofs.Bytecode.PCFast.instructionPC_eq_byteLength]
   rfl
 
-@[simp] theorem fixedPC3893 : Artifact.submissionArtifact.instructionPC 3513 = 4651 := by
+@[simp] theorem fixedPC3893 : Artifact.submissionArtifact.instructionPC 3510 = 4661 := by
   rw [Challenge.Modexp.Submission.Proofs.Bytecode.PCFast.instructionPC_eq_byteLength]
   rfl
 
-@[simp] theorem fixedPC3894 : Artifact.submissionArtifact.instructionPC 3514 = 4652 := by
+@[simp] theorem fixedPC3894 : Artifact.submissionArtifact.instructionPC 3511 = 4662 := by
   rw [Challenge.Modexp.Submission.Proofs.Bytecode.PCFast.instructionPC_eq_byteLength]
   rfl
 
-@[simp] theorem fixedPC3895 : Artifact.submissionArtifact.instructionPC 3515 = 4653 := by
+@[simp] theorem fixedPC3895 : Artifact.submissionArtifact.instructionPC 3512 = 4663 := by
   rw [Challenge.Modexp.Submission.Proofs.Bytecode.PCFast.instructionPC_eq_byteLength]
   rfl
 
-@[simp] theorem fixedPC3896 : Artifact.submissionArtifact.instructionPC 3516 = 4654 := by
+@[simp] theorem fixedPC3896 : Artifact.submissionArtifact.instructionPC 3513 = 4664 := by
   rw [Challenge.Modexp.Submission.Proofs.Bytecode.PCFast.instructionPC_eq_byteLength]
   rfl
 
-@[simp] theorem fixedPC3897 : Artifact.submissionArtifact.instructionPC 3517 = 4655 := by
+@[simp] theorem fixedPC3897 : Artifact.submissionArtifact.instructionPC 3514 = 4665 := by
   rw [Challenge.Modexp.Submission.Proofs.Bytecode.PCFast.instructionPC_eq_byteLength]
   rfl
 
-@[simp] theorem fixedPC3898 : Artifact.submissionArtifact.instructionPC 3518 = 4656 := by
+@[simp] theorem fixedPC3898 : Artifact.submissionArtifact.instructionPC 3515 = 4666 := by
   rw [Challenge.Modexp.Submission.Proofs.Bytecode.PCFast.instructionPC_eq_byteLength]
   rfl
 
-@[simp] theorem fixedPC3899 : Artifact.submissionArtifact.instructionPC 3519 = 4657 := by
+@[simp] theorem fixedPC3899 : Artifact.submissionArtifact.instructionPC 3516 = 4667 := by
   rw [Challenge.Modexp.Submission.Proofs.Bytecode.PCFast.instructionPC_eq_byteLength]
   rfl
 
-@[simp] theorem fixedPC3900 : Artifact.submissionArtifact.instructionPC 3520 = 4658 := by
+@[simp] theorem fixedPC3900 : Artifact.submissionArtifact.instructionPC 3517 = 4668 := by
   rw [Challenge.Modexp.Submission.Proofs.Bytecode.PCFast.instructionPC_eq_byteLength]
   rfl
 
-@[simp] theorem fixedPC3901 : Artifact.submissionArtifact.instructionPC 3521 = 4659 := by
+@[simp] theorem fixedPC3901 : Artifact.submissionArtifact.instructionPC 3518 = 4669 := by
   rw [Challenge.Modexp.Submission.Proofs.Bytecode.PCFast.instructionPC_eq_byteLength]
   rfl
 
-@[simp] theorem fixedPC3902 : Artifact.submissionArtifact.instructionPC 3522 = 4660 := by
+@[simp] theorem fixedPC3902 : Artifact.submissionArtifact.instructionPC 3519 = 4670 := by
   rw [Challenge.Modexp.Submission.Proofs.Bytecode.PCFast.instructionPC_eq_byteLength]
   rfl
 
-@[simp] theorem fixedPC3903 : Artifact.submissionArtifact.instructionPC 3523 = 4661 := by
+@[simp] theorem fixedPC3903 : Artifact.submissionArtifact.instructionPC 3520 = 4671 := by
   rw [Challenge.Modexp.Submission.Proofs.Bytecode.PCFast.instructionPC_eq_byteLength]
   rfl
 
-@[simp] theorem fixedPC3904 : Artifact.submissionArtifact.instructionPC 3524 = 4662 := by
+@[simp] theorem fixedPC3904 : Artifact.submissionArtifact.instructionPC 3521 = 4672 := by
   rw [Challenge.Modexp.Submission.Proofs.Bytecode.PCFast.instructionPC_eq_byteLength]
   rfl
 
-@[simp] theorem fixedPC3905 : Artifact.submissionArtifact.instructionPC 3525 = 4663 := by
+@[simp] theorem fixedPC3905 : Artifact.submissionArtifact.instructionPC 3522 = 4673 := by
   rw [Challenge.Modexp.Submission.Proofs.Bytecode.PCFast.instructionPC_eq_byteLength]
   rfl
 
-@[simp] theorem fixedPC3906 : Artifact.submissionArtifact.instructionPC 3526 = 4664 := by
+@[simp] theorem fixedPC3906 : Artifact.submissionArtifact.instructionPC 3523 = 4674 := by
   rw [Challenge.Modexp.Submission.Proofs.Bytecode.PCFast.instructionPC_eq_byteLength]
   rfl
 
-@[simp] theorem fixedPC3907 : Artifact.submissionArtifact.instructionPC 3527 = 4667 := by
+@[simp] theorem fixedPC3907 : Artifact.submissionArtifact.instructionPC 3524 = 4677 := by
   rw [Challenge.Modexp.Submission.Proofs.Bytecode.PCFast.instructionPC_eq_byteLength]
   rfl
 
-@[simp] theorem fixedPC3908 : Artifact.submissionArtifact.instructionPC 3528 = 4668 := by
+@[simp] theorem fixedPC3908 : Artifact.submissionArtifact.instructionPC 3525 = 4678 := by
   rw [Challenge.Modexp.Submission.Proofs.Bytecode.PCFast.instructionPC_eq_byteLength]
   rfl
 
-@[simp] theorem fixedPC3909 : Artifact.submissionArtifact.instructionPC 3529 = 4671 := by
+@[simp] theorem fixedPC3909 : Artifact.submissionArtifact.instructionPC 3526 = 4681 := by
   rw [Challenge.Modexp.Submission.Proofs.Bytecode.PCFast.instructionPC_eq_byteLength]
   rfl
 
-@[simp] theorem fixedPC3910 : Artifact.submissionArtifact.instructionPC 3530 = 4672 := by
+@[simp] theorem fixedPC3910 : Artifact.submissionArtifact.instructionPC 3527 = 4682 := by
   rw [Challenge.Modexp.Submission.Proofs.Bytecode.PCFast.instructionPC_eq_byteLength]
   rfl
 
-@[simp] theorem fixedPC3911 : Artifact.submissionArtifact.instructionPC 3531 = 4674 := by
+@[simp] theorem fixedPC3911 : Artifact.submissionArtifact.instructionPC 3528 = 4684 := by
   rw [Challenge.Modexp.Submission.Proofs.Bytecode.PCFast.instructionPC_eq_byteLength]
   rfl
 
-@[simp] theorem fixedPC3912 : Artifact.submissionArtifact.instructionPC 3532 = 4675 := by
+@[simp] theorem fixedPC3912 : Artifact.submissionArtifact.instructionPC 3529 = 4685 := by
   rw [Challenge.Modexp.Submission.Proofs.Bytecode.PCFast.instructionPC_eq_byteLength]
   rfl
 
-@[simp] theorem fixedPC3913 : Artifact.submissionArtifact.instructionPC 3533 = 4676 := by
+@[simp] theorem fixedPC3913 : Artifact.submissionArtifact.instructionPC 3530 = 4686 := by
   rw [Challenge.Modexp.Submission.Proofs.Bytecode.PCFast.instructionPC_eq_byteLength]
   rfl
 
-@[simp] theorem fixedPC3914 : Artifact.submissionArtifact.instructionPC 3534 = 4677 := by
+@[simp] theorem fixedPC3914 : Artifact.submissionArtifact.instructionPC 3531 = 4687 := by
   rw [Challenge.Modexp.Submission.Proofs.Bytecode.PCFast.instructionPC_eq_byteLength]
   rfl
 
-@[simp] theorem fixedPC3915 : Artifact.submissionArtifact.instructionPC 3535 = 4678 := by
+@[simp] theorem fixedPC3915 : Artifact.submissionArtifact.instructionPC 3532 = 4688 := by
   rw [Challenge.Modexp.Submission.Proofs.Bytecode.PCFast.instructionPC_eq_byteLength]
   rfl
 
-@[simp] theorem fixedPC3916 : Artifact.submissionArtifact.instructionPC 3536 = 4679 := by
+@[simp] theorem fixedPC3916 : Artifact.submissionArtifact.instructionPC 3533 = 4689 := by
   rw [Challenge.Modexp.Submission.Proofs.Bytecode.PCFast.instructionPC_eq_byteLength]
   rfl
 
-@[simp] theorem fixedPC3917 : Artifact.submissionArtifact.instructionPC 3537 = 4680 := by
+@[simp] theorem fixedPC3917 : Artifact.submissionArtifact.instructionPC 3534 = 4690 := by
   rw [Challenge.Modexp.Submission.Proofs.Bytecode.PCFast.instructionPC_eq_byteLength]
   rfl
 
-@[simp] theorem fixedPC3918 : Artifact.submissionArtifact.instructionPC 3538 = 4681 := by
+@[simp] theorem fixedPC3918 : Artifact.submissionArtifact.instructionPC 3535 = 4691 := by
   rw [Challenge.Modexp.Submission.Proofs.Bytecode.PCFast.instructionPC_eq_byteLength]
   rfl
 
-@[simp] theorem fixedPC3919 : Artifact.submissionArtifact.instructionPC 3539 = 4682 := by
+@[simp] theorem fixedPC3919 : Artifact.submissionArtifact.instructionPC 3536 = 4692 := by
   rw [Challenge.Modexp.Submission.Proofs.Bytecode.PCFast.instructionPC_eq_byteLength]
   rfl
 
-@[simp] theorem fixedPC3920 : Artifact.submissionArtifact.instructionPC 3540 = 4683 := by
+@[simp] theorem fixedPC3920 : Artifact.submissionArtifact.instructionPC 3537 = 4693 := by
   rw [Challenge.Modexp.Submission.Proofs.Bytecode.PCFast.instructionPC_eq_byteLength]
   rfl
 
-@[simp] theorem fixedPC3921 : Artifact.submissionArtifact.instructionPC 3541 = 4684 := by
+@[simp] theorem fixedPC3921 : Artifact.submissionArtifact.instructionPC 3538 = 4694 := by
   rw [Challenge.Modexp.Submission.Proofs.Bytecode.PCFast.instructionPC_eq_byteLength]
   rfl
 
-@[simp] theorem fixedPC3922 : Artifact.submissionArtifact.instructionPC 3542 = 4685 := by
+@[simp] theorem fixedPC3922 : Artifact.submissionArtifact.instructionPC 3539 = 4695 := by
   rw [Challenge.Modexp.Submission.Proofs.Bytecode.PCFast.instructionPC_eq_byteLength]
   rfl
 
-@[simp] theorem fixedPC3923 : Artifact.submissionArtifact.instructionPC 3543 = 4686 := by
+@[simp] theorem fixedPC3923 : Artifact.submissionArtifact.instructionPC 3540 = 4696 := by
   rw [Challenge.Modexp.Submission.Proofs.Bytecode.PCFast.instructionPC_eq_byteLength]
   rfl
 
-@[simp] theorem fixedPC3924 : Artifact.submissionArtifact.instructionPC 3544 = 4687 := by
+@[simp] theorem fixedPC3924 : Artifact.submissionArtifact.instructionPC 3541 = 4697 := by
   rw [Challenge.Modexp.Submission.Proofs.Bytecode.PCFast.instructionPC_eq_byteLength]
   rfl
 
-@[simp] theorem fixedPC3925 : Artifact.submissionArtifact.instructionPC 3545 = 4690 := by
+@[simp] theorem fixedPC3925 : Artifact.submissionArtifact.instructionPC 3542 = 4700 := by
   rw [Challenge.Modexp.Submission.Proofs.Bytecode.PCFast.instructionPC_eq_byteLength]
   rfl
 
-@[simp] theorem fixedPC3926 : Artifact.submissionArtifact.instructionPC 3546 = 4691 := by
+@[simp] theorem fixedPC3926 : Artifact.submissionArtifact.instructionPC 3543 = 4701 := by
   rw [Challenge.Modexp.Submission.Proofs.Bytecode.PCFast.instructionPC_eq_byteLength]
   rfl
 
-@[simp] theorem fixedPC3927 : Artifact.submissionArtifact.instructionPC 3547 = 4694 := by
+@[simp] theorem fixedPC3927 : Artifact.submissionArtifact.instructionPC 3544 = 4704 := by
   rw [Challenge.Modexp.Submission.Proofs.Bytecode.PCFast.instructionPC_eq_byteLength]
   rfl
 
-@[simp] theorem fixedPC3928 : Artifact.submissionArtifact.instructionPC 3548 = 4695 := by
+@[simp] theorem fixedPC3928 : Artifact.submissionArtifact.instructionPC 3545 = 4705 := by
   rw [Challenge.Modexp.Submission.Proofs.Bytecode.PCFast.instructionPC_eq_byteLength]
   rfl
 
-@[simp] theorem fixedPC3929 : Artifact.submissionArtifact.instructionPC 3549 = 4696 := by
+@[simp] theorem fixedPC3929 : Artifact.submissionArtifact.instructionPC 3546 = 4706 := by
   rw [Challenge.Modexp.Submission.Proofs.Bytecode.PCFast.instructionPC_eq_byteLength]
   rfl
 
-@[simp] theorem fixedPC3930 : Artifact.submissionArtifact.instructionPC 3550 = 4697 := by
+@[simp] theorem fixedPC3930 : Artifact.submissionArtifact.instructionPC 3547 = 4707 := by
   rw [Challenge.Modexp.Submission.Proofs.Bytecode.PCFast.instructionPC_eq_byteLength]
   rfl
 
-@[simp] theorem fixedPC3931 : Artifact.submissionArtifact.instructionPC 3551 = 4698 := by
+@[simp] theorem fixedPC3931 : Artifact.submissionArtifact.instructionPC 3548 = 4708 := by
   rw [Challenge.Modexp.Submission.Proofs.Bytecode.PCFast.instructionPC_eq_byteLength]
   rfl
 
-@[simp] theorem fixedPC3932 : Artifact.submissionArtifact.instructionPC 3552 = 4699 := by
+@[simp] theorem fixedPC3932 : Artifact.submissionArtifact.instructionPC 3549 = 4709 := by
   rw [Challenge.Modexp.Submission.Proofs.Bytecode.PCFast.instructionPC_eq_byteLength]
   rfl
 
-@[simp] theorem fixedPC3933 : Artifact.submissionArtifact.instructionPC 3553 = 4700 := by
+@[simp] theorem fixedPC3933 : Artifact.submissionArtifact.instructionPC 3550 = 4710 := by
   rw [Challenge.Modexp.Submission.Proofs.Bytecode.PCFast.instructionPC_eq_byteLength]
   rfl
 
-@[simp] theorem fixedPC3934 : Artifact.submissionArtifact.instructionPC 3554 = 4701 := by
+@[simp] theorem fixedPC3934 : Artifact.submissionArtifact.instructionPC 3551 = 4711 := by
   rw [Challenge.Modexp.Submission.Proofs.Bytecode.PCFast.instructionPC_eq_byteLength]
   rfl
 
-@[simp] theorem fixedPC3935 : Artifact.submissionArtifact.instructionPC 3555 = 4702 := by
+@[simp] theorem fixedPC3935 : Artifact.submissionArtifact.instructionPC 3552 = 4712 := by
   rw [Challenge.Modexp.Submission.Proofs.Bytecode.PCFast.instructionPC_eq_byteLength]
   rfl
 
-@[simp] theorem fixedPC3936 : Artifact.submissionArtifact.instructionPC 3556 = 4703 := by
+@[simp] theorem fixedPC3936 : Artifact.submissionArtifact.instructionPC 3553 = 4713 := by
   rw [Challenge.Modexp.Submission.Proofs.Bytecode.PCFast.instructionPC_eq_byteLength]
   rfl
 
-@[simp] theorem fixedPC3937 : Artifact.submissionArtifact.instructionPC 3557 = 4704 := by
+@[simp] theorem fixedPC3937 : Artifact.submissionArtifact.instructionPC 3554 = 4714 := by
   rw [Challenge.Modexp.Submission.Proofs.Bytecode.PCFast.instructionPC_eq_byteLength]
   rfl
 
-@[simp] theorem fixedPC3938 : Artifact.submissionArtifact.instructionPC 3558 = 4705 := by
+@[simp] theorem fixedPC3938 : Artifact.submissionArtifact.instructionPC 3555 = 4715 := by
   rw [Challenge.Modexp.Submission.Proofs.Bytecode.PCFast.instructionPC_eq_byteLength]
   rfl
 
-@[simp] theorem fixedPC3939 : Artifact.submissionArtifact.instructionPC 3559 = 4706 := by
+@[simp] theorem fixedPC3939 : Artifact.submissionArtifact.instructionPC 3556 = 4716 := by
   rw [Challenge.Modexp.Submission.Proofs.Bytecode.PCFast.instructionPC_eq_byteLength]
   rfl
 
-@[simp] theorem fixedPC3940 : Artifact.submissionArtifact.instructionPC 3560 = 4707 := by
+@[simp] theorem fixedPC3940 : Artifact.submissionArtifact.instructionPC 3557 = 4717 := by
   rw [Challenge.Modexp.Submission.Proofs.Bytecode.PCFast.instructionPC_eq_byteLength]
   rfl
 
-@[simp] theorem fixedPC3941 : Artifact.submissionArtifact.instructionPC 3561 = 4708 := by
+@[simp] theorem fixedPC3941 : Artifact.submissionArtifact.instructionPC 3558 = 4718 := by
   rw [Challenge.Modexp.Submission.Proofs.Bytecode.PCFast.instructionPC_eq_byteLength]
   rfl
 
-@[simp] theorem fixedPC3942 : Artifact.submissionArtifact.instructionPC 3562 = 4709 := by
+@[simp] theorem fixedPC3942 : Artifact.submissionArtifact.instructionPC 3559 = 4719 := by
   rw [Challenge.Modexp.Submission.Proofs.Bytecode.PCFast.instructionPC_eq_byteLength]
   rfl
 
-@[simp] theorem fixedPC3943 : Artifact.submissionArtifact.instructionPC 3563 = 4712 := by
+@[simp] theorem fixedPC3943 : Artifact.submissionArtifact.instructionPC 3560 = 4722 := by
   rw [Challenge.Modexp.Submission.Proofs.Bytecode.PCFast.instructionPC_eq_byteLength]
   rfl
 
-@[simp] theorem fixedPC3944 : Artifact.submissionArtifact.instructionPC 3564 = 4713 := by
+@[simp] theorem fixedPC3944 : Artifact.submissionArtifact.instructionPC 3561 = 4723 := by
   rw [Challenge.Modexp.Submission.Proofs.Bytecode.PCFast.instructionPC_eq_byteLength]
   rfl
 
-@[simp] theorem fixedPC3945 : Artifact.submissionArtifact.instructionPC 3565 = 4714 := by
+@[simp] theorem fixedPC3945 : Artifact.submissionArtifact.instructionPC 3562 = 4724 := by
   rw [Challenge.Modexp.Submission.Proofs.Bytecode.PCFast.instructionPC_eq_byteLength]
   rfl
 
-@[simp] theorem fixedPC3946 : Artifact.submissionArtifact.instructionPC 3566 = 4717 := by
+@[simp] theorem fixedPC3946 : Artifact.submissionArtifact.instructionPC 3563 = 4727 := by
   rw [Challenge.Modexp.Submission.Proofs.Bytecode.PCFast.instructionPC_eq_byteLength]
   rfl
 
-@[simp] theorem fixedPC3947 : Artifact.submissionArtifact.instructionPC 3567 = 4718 := by
+@[simp] theorem fixedPC3947 : Artifact.submissionArtifact.instructionPC 3564 = 4728 := by
   rw [Challenge.Modexp.Submission.Proofs.Bytecode.PCFast.instructionPC_eq_byteLength]
   rfl
 
-@[simp] theorem fixedPC3948 : Artifact.submissionArtifact.instructionPC 3568 = 4719 := by
+@[simp] theorem fixedPC3948 : Artifact.submissionArtifact.instructionPC 3565 = 4729 := by
   rw [Challenge.Modexp.Submission.Proofs.Bytecode.PCFast.instructionPC_eq_byteLength]
   rfl
 
-@[simp] theorem fixedPC3949 : Artifact.submissionArtifact.instructionPC 3585 = 4748 := by
+@[simp] theorem fixedPC3949 : Artifact.submissionArtifact.instructionPC 3582 = 4758 := by
   rw [Challenge.Modexp.Submission.Proofs.Bytecode.PCFast.instructionPC_eq_byteLength]
   rfl
 
-@[simp] theorem fixedPC3950 : Artifact.submissionArtifact.instructionPC 3585 = 4748 :=
+@[simp] theorem fixedPC3950 : Artifact.submissionArtifact.instructionPC 3582 = 4758 :=
   fixedPC3949
 
-@[simp] theorem fixedPC3951 : Artifact.submissionArtifact.instructionPC 3586 = 4749 := by
+@[simp] theorem fixedPC3951 : Artifact.submissionArtifact.instructionPC 3583 = 4759 := by
   rw [Challenge.Modexp.Submission.Proofs.Bytecode.PCFast.instructionPC_eq_byteLength]
   rfl
 
-@[simp] theorem fixedPC3952 : Artifact.submissionArtifact.instructionPC 3587 = 4752 := by
+@[simp] theorem fixedPC3952 : Artifact.submissionArtifact.instructionPC 3584 = 4762 := by
   rw [Challenge.Modexp.Submission.Proofs.Bytecode.PCFast.instructionPC_eq_byteLength]
   rfl
 
-@[simp] theorem fixedPC3953 : Artifact.submissionArtifact.instructionPC 3588 = 4753 := by
+@[simp] theorem fixedPC3953 : Artifact.submissionArtifact.instructionPC 3585 = 4763 := by
   rw [Challenge.Modexp.Submission.Proofs.Bytecode.PCFast.instructionPC_eq_byteLength]
   rfl
 
-@[simp] theorem fixedPC3954 : Artifact.submissionArtifact.instructionPC 3589 = 4756 := by
+@[simp] theorem fixedPC3954 : Artifact.submissionArtifact.instructionPC 3586 = 4766 := by
   rw [Challenge.Modexp.Submission.Proofs.Bytecode.PCFast.instructionPC_eq_byteLength]
   rfl
 
-@[simp] theorem fixedPC3955 : Artifact.submissionArtifact.instructionPC 3590 = 4757 := by
+@[simp] theorem fixedPC3955 : Artifact.submissionArtifact.instructionPC 3587 = 4767 := by
   rw [Challenge.Modexp.Submission.Proofs.Bytecode.PCFast.instructionPC_eq_byteLength]
   rfl
 
-@[simp] theorem fixedPC3956 : Artifact.submissionArtifact.instructionPC 3591 = 4758 := by
+@[simp] theorem fixedPC3956 : Artifact.submissionArtifact.instructionPC 3588 = 4768 := by
   rw [Challenge.Modexp.Submission.Proofs.Bytecode.PCFast.instructionPC_eq_byteLength]
   rfl
 
-@[simp] theorem fixedPC3957 : Artifact.submissionArtifact.instructionPC 3592 = 4759 := by
+@[simp] theorem fixedPC3957 : Artifact.submissionArtifact.instructionPC 3589 = 4769 := by
   rw [Challenge.Modexp.Submission.Proofs.Bytecode.PCFast.instructionPC_eq_byteLength]
   rfl
 
@@ -1236,226 +1236,226 @@ def csFixedTail4 : List (Challenge.EvmProof.Stepper.Located Artifact.submissionA
   rw [Challenge.Modexp.Submission.Proofs.Bytecode.PCFast.instructionPC_eq_byteLength]
   rfl
 
-@[simp] theorem fixedPC3999 : Artifact.submissionArtifact.instructionPC 3299 = 4351 := by
+@[simp] theorem fixedPC3999 : Artifact.submissionArtifact.instructionPC 3287 = 4346 := by
   rw [Challenge.Modexp.Submission.Proofs.Bytecode.PCFast.instructionPC_eq_byteLength]
   rfl
 
-@[simp] theorem fixedJump5280 : Decode.isValidJumpDest Challenge.Modexp.submissionBytecode 4351 = true := by
-  simpa only [Artifact.instructionPC, fixedPC3999] using Artifact.isValidJumpDest_index 3299 (by rfl)
+@[simp] theorem fixedJump5280 : Decode.isValidJumpDest Challenge.Modexp.submissionBytecode 4346 = true := by
+  simpa only [Artifact.instructionPC, fixedPC3999] using Artifact.isValidJumpDest_index 3287 (by rfl)
 
-@[simp] theorem fixedPC4000 : Artifact.submissionArtifact.instructionPC 3300 = 4352 := by
+@[simp] theorem fixedPC4000 : Artifact.submissionArtifact.instructionPC 3288 = 4347 := by
   rw [Challenge.Modexp.Submission.Proofs.Bytecode.PCFast.instructionPC_eq_byteLength]
   rfl
 
-@[simp] theorem fixedPC4001 : Artifact.submissionArtifact.instructionPC 3301 = 4355 := by
+@[simp] theorem fixedPC4001 : Artifact.submissionArtifact.instructionPC 3289 = 4350 := by
   rw [Challenge.Modexp.Submission.Proofs.Bytecode.PCFast.instructionPC_eq_byteLength]
   rfl
 
-@[simp] theorem fixedPC4002 : Artifact.submissionArtifact.instructionPC 3302 = 4356 := by
+@[simp] theorem fixedPC4002 : Artifact.submissionArtifact.instructionPC 3290 = 4351 := by
   rw [Challenge.Modexp.Submission.Proofs.Bytecode.PCFast.instructionPC_eq_byteLength]
   rfl
 
-@[simp] theorem fixedPC4003 : Artifact.submissionArtifact.instructionPC 3303 = 4358 := by
+@[simp] theorem fixedPC4003 : Artifact.submissionArtifact.instructionPC 3291 = 4353 := by
   rw [Challenge.Modexp.Submission.Proofs.Bytecode.PCFast.instructionPC_eq_byteLength]
   rfl
 
-@[simp] theorem fixedPC4004 : Artifact.submissionArtifact.instructionPC 3304 = 4359 := by
+@[simp] theorem fixedPC4004 : Artifact.submissionArtifact.instructionPC 3292 = 4354 := by
   rw [Challenge.Modexp.Submission.Proofs.Bytecode.PCFast.instructionPC_eq_byteLength]
   rfl
 
-@[simp] theorem fixedPC4005 : Artifact.submissionArtifact.instructionPC 3305 = 4360 := by
+@[simp] theorem fixedPC4005 : Artifact.submissionArtifact.instructionPC 3293 = 4355 := by
   rw [Challenge.Modexp.Submission.Proofs.Bytecode.PCFast.instructionPC_eq_byteLength]
   rfl
 
-@[simp] theorem fixedPC4006 : Artifact.submissionArtifact.instructionPC 3306 = 4361 := by
+@[simp] theorem fixedPC4006 : Artifact.submissionArtifact.instructionPC 3294 = 4356 := by
   rw [Challenge.Modexp.Submission.Proofs.Bytecode.PCFast.instructionPC_eq_byteLength]
   rfl
 
-@[simp] theorem fixedPC4007 : Artifact.submissionArtifact.instructionPC 3307 = 4362 := by
+@[simp] theorem fixedPC4007 : Artifact.submissionArtifact.instructionPC 3295 = 4357 := by
   rw [Challenge.Modexp.Submission.Proofs.Bytecode.PCFast.instructionPC_eq_byteLength]
   rfl
 
-@[simp] theorem fixedPC4008 : Artifact.submissionArtifact.instructionPC 3308 = 4363 := by
+@[simp] theorem fixedPC4008 : Artifact.submissionArtifact.instructionPC 3296 = 4358 := by
   rw [Challenge.Modexp.Submission.Proofs.Bytecode.PCFast.instructionPC_eq_byteLength]
   rfl
 
-@[simp] theorem fixedPC4009 : Artifact.submissionArtifact.instructionPC 3309 = 4364 := by
+@[simp] theorem fixedPC4009 : Artifact.submissionArtifact.instructionPC 3297 = 4359 := by
   rw [Challenge.Modexp.Submission.Proofs.Bytecode.PCFast.instructionPC_eq_byteLength]
   rfl
 
-@[simp] theorem fixedPC4010 : Artifact.submissionArtifact.instructionPC 3310 = 4367 := by
+@[simp] theorem fixedPC4010 : Artifact.submissionArtifact.instructionPC 3298 = 4362 := by
   rw [Challenge.Modexp.Submission.Proofs.Bytecode.PCFast.instructionPC_eq_byteLength]
   rfl
 
-@[simp] theorem fixedPC4011 : Artifact.submissionArtifact.instructionPC 3311 = 4368 := by
+@[simp] theorem fixedPC4011 : Artifact.submissionArtifact.instructionPC 3299 = 4363 := by
   rw [Challenge.Modexp.Submission.Proofs.Bytecode.PCFast.instructionPC_eq_byteLength]
   rfl
 
-@[simp] theorem fixedPC4012 : Artifact.submissionArtifact.instructionPC 3312 = 4371 := by
+@[simp] theorem fixedPC4012 : Artifact.submissionArtifact.instructionPC 3300 = 4366 := by
   rw [Challenge.Modexp.Submission.Proofs.Bytecode.PCFast.instructionPC_eq_byteLength]
   rfl
 
-@[simp] theorem earlyExtraPC2880 : Artifact.submissionArtifact.instructionPC 2488 = 3306 := by
+@[simp] theorem earlyExtraPC2880 : Artifact.submissionArtifact.instructionPC 2475 = 3300 := by
   rw [Challenge.Modexp.Submission.Proofs.Bytecode.PCFast.instructionPC_eq_byteLength]
   rfl
 
-@[simp] theorem earlyExtraPC2883 : Artifact.submissionArtifact.instructionPC 3286 = 4330 := by
+@[simp] theorem earlyExtraPC2883 : Artifact.submissionArtifact.instructionPC 3274 = 4325 := by
   rw [Challenge.Modexp.Submission.Proofs.Bytecode.PCFast.instructionPC_eq_byteLength]
   rfl
 
-@[simp] theorem earlyExtraPC2884 : Artifact.submissionArtifact.instructionPC 3287 = 4331 := by
+@[simp] theorem earlyExtraPC2884 : Artifact.submissionArtifact.instructionPC 3275 = 4326 := by
   rw [Challenge.Modexp.Submission.Proofs.Bytecode.PCFast.instructionPC_eq_byteLength]
   rfl
 
-@[simp] theorem earlyExtraPC2885 : Artifact.submissionArtifact.instructionPC 3288 = 4332 := by
+@[simp] theorem earlyExtraPC2885 : Artifact.submissionArtifact.instructionPC 3276 = 4327 := by
   rw [Challenge.Modexp.Submission.Proofs.Bytecode.PCFast.instructionPC_eq_byteLength]
   rfl
 
-@[simp] theorem earlyExtraPC2886 : Artifact.submissionArtifact.instructionPC 3289 = 4333 := by
+@[simp] theorem earlyExtraPC2886 : Artifact.submissionArtifact.instructionPC 3277 = 4328 := by
   rw [Challenge.Modexp.Submission.Proofs.Bytecode.PCFast.instructionPC_eq_byteLength]
   rfl
 
-@[simp] theorem earlyExtraPC2887 : Artifact.submissionArtifact.instructionPC 3290 = 4336 := by
+@[simp] theorem earlyExtraPC2887 : Artifact.submissionArtifact.instructionPC 3278 = 4331 := by
   rw [Challenge.Modexp.Submission.Proofs.Bytecode.PCFast.instructionPC_eq_byteLength]
   rfl
 
-@[simp] theorem earlyExtraPC2888 : Artifact.submissionArtifact.instructionPC 3291 = 4337 := by
+@[simp] theorem earlyExtraPC2888 : Artifact.submissionArtifact.instructionPC 3279 = 4332 := by
   rw [Challenge.Modexp.Submission.Proofs.Bytecode.PCFast.instructionPC_eq_byteLength]
   rfl
 
-@[simp] theorem earlyExtraPC2889 : Artifact.submissionArtifact.instructionPC 3292 = 4338 := by
+@[simp] theorem earlyExtraPC2889 : Artifact.submissionArtifact.instructionPC 3280 = 4333 := by
   rw [Challenge.Modexp.Submission.Proofs.Bytecode.PCFast.instructionPC_eq_byteLength]
   rfl
 
-@[simp] theorem earlyExtraPC2890 : Artifact.submissionArtifact.instructionPC 3293 = 4341 := by
+@[simp] theorem earlyExtraPC2890 : Artifact.submissionArtifact.instructionPC 3281 = 4336 := by
   rw [Challenge.Modexp.Submission.Proofs.Bytecode.PCFast.instructionPC_eq_byteLength]
   rfl
 
-@[simp] theorem earlyExtraPC2891 : Artifact.submissionArtifact.instructionPC 3294 = 4342 := by
+@[simp] theorem earlyExtraPC2891 : Artifact.submissionArtifact.instructionPC 3282 = 4337 := by
   rw [Challenge.Modexp.Submission.Proofs.Bytecode.PCFast.instructionPC_eq_byteLength]
   rfl
 
-@[simp] theorem earlyExtraPC2892 : Artifact.submissionArtifact.instructionPC 3295 = 4343 := by
+@[simp] theorem earlyExtraPC2892 : Artifact.submissionArtifact.instructionPC 3283 = 4338 := by
   rw [Challenge.Modexp.Submission.Proofs.Bytecode.PCFast.instructionPC_eq_byteLength]
   rfl
 
-@[simp] theorem earlyExtraPC2893 : Artifact.submissionArtifact.instructionPC 3295 = 4343 := by
+@[simp] theorem earlyExtraPC2893 : Artifact.submissionArtifact.instructionPC 3283 = 4338 := by
   rw [Challenge.Modexp.Submission.Proofs.Bytecode.PCFast.instructionPC_eq_byteLength]
   rfl
 
-@[simp] theorem earlyExtraPC2894 : Artifact.submissionArtifact.instructionPC 3296 = 4346 := by
+@[simp] theorem earlyExtraPC2894 : Artifact.submissionArtifact.instructionPC 3284 = 4341 := by
   rw [Challenge.Modexp.Submission.Proofs.Bytecode.PCFast.instructionPC_eq_byteLength]
   rfl
 
-@[simp] theorem earlyExtraPC2895 : Artifact.submissionArtifact.instructionPC 3297 = 4347 := by
+@[simp] theorem earlyExtraPC2895 : Artifact.submissionArtifact.instructionPC 3285 = 4342 := by
   rw [Challenge.Modexp.Submission.Proofs.Bytecode.PCFast.instructionPC_eq_byteLength]
   rfl
 
-@[simp] theorem earlyExtraPC2896 : Artifact.submissionArtifact.instructionPC 3298 = 4350 := by
+@[simp] theorem earlyExtraPC2896 : Artifact.submissionArtifact.instructionPC 3286 = 4345 := by
   rw [Challenge.Modexp.Submission.Proofs.Bytecode.PCFast.instructionPC_eq_byteLength]
   rfl
 
-@[simp] theorem earlyExtraPC2927 : Artifact.submissionArtifact.instructionPC 2488 = 3306 := by
+@[simp] theorem earlyExtraPC2927 : Artifact.submissionArtifact.instructionPC 2475 = 3300 := by
   rw [Challenge.Modexp.Submission.Proofs.Bytecode.PCFast.instructionPC_eq_byteLength]
   rfl
 
-@[simp] theorem earlyExtraPC2930 : Artifact.submissionArtifact.instructionPC 3299 = 4351 := by
+@[simp] theorem earlyExtraPC2930 : Artifact.submissionArtifact.instructionPC 3287 = 4346 := by
   rw [Challenge.Modexp.Submission.Proofs.Bytecode.PCFast.instructionPC_eq_byteLength]
   rfl
 
-@[simp] theorem earlyExtraPC2931 : Artifact.submissionArtifact.instructionPC 3300 = 4352 := by
+@[simp] theorem earlyExtraPC2931 : Artifact.submissionArtifact.instructionPC 3288 = 4347 := by
   rw [Challenge.Modexp.Submission.Proofs.Bytecode.PCFast.instructionPC_eq_byteLength]
   rfl
 
-@[simp] theorem earlyExtraPC2932 : Artifact.submissionArtifact.instructionPC 3301 = 4355 := by
+@[simp] theorem earlyExtraPC2932 : Artifact.submissionArtifact.instructionPC 3289 = 4350 := by
   rw [Challenge.Modexp.Submission.Proofs.Bytecode.PCFast.instructionPC_eq_byteLength]
   rfl
 
-@[simp] theorem earlyExtraPC2933 : Artifact.submissionArtifact.instructionPC 3302 = 4356 := by
+@[simp] theorem earlyExtraPC2933 : Artifact.submissionArtifact.instructionPC 3290 = 4351 := by
   rw [Challenge.Modexp.Submission.Proofs.Bytecode.PCFast.instructionPC_eq_byteLength]
   rfl
 
-@[simp] theorem earlyExtraPC2934 : Artifact.submissionArtifact.instructionPC 3303 = 4358 := by
+@[simp] theorem earlyExtraPC2934 : Artifact.submissionArtifact.instructionPC 3291 = 4353 := by
   rw [Challenge.Modexp.Submission.Proofs.Bytecode.PCFast.instructionPC_eq_byteLength]
   rfl
 
-@[simp] theorem earlyExtraPC2935 : Artifact.submissionArtifact.instructionPC 3304 = 4359 := by
+@[simp] theorem earlyExtraPC2935 : Artifact.submissionArtifact.instructionPC 3292 = 4354 := by
   rw [Challenge.Modexp.Submission.Proofs.Bytecode.PCFast.instructionPC_eq_byteLength]
   rfl
 
-@[simp] theorem earlyExtraPC2936 : Artifact.submissionArtifact.instructionPC 3305 = 4360 := by
+@[simp] theorem earlyExtraPC2936 : Artifact.submissionArtifact.instructionPC 3293 = 4355 := by
   rw [Challenge.Modexp.Submission.Proofs.Bytecode.PCFast.instructionPC_eq_byteLength]
   rfl
 
-@[simp] theorem earlyExtraPC2937 : Artifact.submissionArtifact.instructionPC 3306 = 4361 := by
+@[simp] theorem earlyExtraPC2937 : Artifact.submissionArtifact.instructionPC 3294 = 4356 := by
   rw [Challenge.Modexp.Submission.Proofs.Bytecode.PCFast.instructionPC_eq_byteLength]
   rfl
 
-@[simp] theorem earlyExtraPC2938 : Artifact.submissionArtifact.instructionPC 3307 = 4362 := by
+@[simp] theorem earlyExtraPC2938 : Artifact.submissionArtifact.instructionPC 3295 = 4357 := by
   rw [Challenge.Modexp.Submission.Proofs.Bytecode.PCFast.instructionPC_eq_byteLength]
   rfl
 
-@[simp] theorem earlyExtraPC2939 : Artifact.submissionArtifact.instructionPC 3308 = 4363 := by
+@[simp] theorem earlyExtraPC2939 : Artifact.submissionArtifact.instructionPC 3296 = 4358 := by
   rw [Challenge.Modexp.Submission.Proofs.Bytecode.PCFast.instructionPC_eq_byteLength]
   rfl
 
-@[simp] theorem earlyExtraPC2940 : Artifact.submissionArtifact.instructionPC 3309 = 4364 := by
+@[simp] theorem earlyExtraPC2940 : Artifact.submissionArtifact.instructionPC 3297 = 4359 := by
   rw [Challenge.Modexp.Submission.Proofs.Bytecode.PCFast.instructionPC_eq_byteLength]
   rfl
 
-@[simp] theorem earlyExtraPC2941 : Artifact.submissionArtifact.instructionPC 3310 = 4367 := by
+@[simp] theorem earlyExtraPC2941 : Artifact.submissionArtifact.instructionPC 3298 = 4362 := by
   rw [Challenge.Modexp.Submission.Proofs.Bytecode.PCFast.instructionPC_eq_byteLength]
   rfl
 
-@[simp] theorem earlyExtraPC2942 : Artifact.submissionArtifact.instructionPC 3311 = 4368 := by
+@[simp] theorem earlyExtraPC2942 : Artifact.submissionArtifact.instructionPC 3299 = 4363 := by
   rw [Challenge.Modexp.Submission.Proofs.Bytecode.PCFast.instructionPC_eq_byteLength]
   rfl
 
-@[simp] theorem earlyExtraPC2943 : Artifact.submissionArtifact.instructionPC 3312 = 4371 := by
+@[simp] theorem earlyExtraPC2943 : Artifact.submissionArtifact.instructionPC 3300 = 4366 := by
   rw [Challenge.Modexp.Submission.Proofs.Bytecode.PCFast.instructionPC_eq_byteLength]
   rfl
 
-@[simp] theorem earlyExtraPC3918 : Artifact.submissionArtifact.instructionPC 3569 = 4722 := by
+@[simp] theorem earlyExtraPC3918 : Artifact.submissionArtifact.instructionPC 3566 = 4732 := by
   rw [Challenge.Modexp.Submission.Proofs.Bytecode.PCFast.instructionPC_eq_byteLength]
   rfl
 
-@[simp] theorem earlyExtraPC3919 : Artifact.submissionArtifact.instructionPC 3570 = 4723 := by
+@[simp] theorem earlyExtraPC3919 : Artifact.submissionArtifact.instructionPC 3567 = 4733 := by
   rw [Challenge.Modexp.Submission.Proofs.Bytecode.PCFast.instructionPC_eq_byteLength]
   rfl
 
-@[simp] theorem earlyExtraPC3920 : Artifact.submissionArtifact.instructionPC 3571 = 4726 := by
+@[simp] theorem earlyExtraPC3920 : Artifact.submissionArtifact.instructionPC 3568 = 4736 := by
   rw [Challenge.Modexp.Submission.Proofs.Bytecode.PCFast.instructionPC_eq_byteLength]
   rfl
 
-@[simp] theorem earlyExtraPC3921 : Artifact.submissionArtifact.instructionPC 3577 = 4736 := by
+@[simp] theorem earlyExtraPC3921 : Artifact.submissionArtifact.instructionPC 3574 = 4746 := by
   rw [Challenge.Modexp.Submission.Proofs.Bytecode.PCFast.instructionPC_eq_byteLength]
   rfl
 
-@[simp] theorem earlyExtraPC3922 : Artifact.submissionArtifact.instructionPC 3578 = 4737 := by
+@[simp] theorem earlyExtraPC3922 : Artifact.submissionArtifact.instructionPC 3575 = 4747 := by
   rw [Challenge.Modexp.Submission.Proofs.Bytecode.PCFast.instructionPC_eq_byteLength]
   rfl
 
-@[simp] theorem earlyExtraPC3923 : Artifact.submissionArtifact.instructionPC 3579 = 4740 := by
+@[simp] theorem earlyExtraPC3923 : Artifact.submissionArtifact.instructionPC 3576 = 4750 := by
   rw [Challenge.Modexp.Submission.Proofs.Bytecode.PCFast.instructionPC_eq_byteLength]
   rfl
 
-@[simp] theorem earlyExtraPC3924 : Artifact.submissionArtifact.instructionPC 3580 = 4743 := by
+@[simp] theorem earlyExtraPC3924 : Artifact.submissionArtifact.instructionPC 3577 = 4753 := by
   rw [Challenge.Modexp.Submission.Proofs.Bytecode.PCFast.instructionPC_eq_byteLength]
   rfl
 
-@[simp] theorem earlyExtraPC3925 : Artifact.submissionArtifact.instructionPC 3581 = 4744 := by
+@[simp] theorem earlyExtraPC3925 : Artifact.submissionArtifact.instructionPC 3578 = 4754 := by
   rw [Challenge.Modexp.Submission.Proofs.Bytecode.PCFast.instructionPC_eq_byteLength]
   rfl
 
-@[simp] theorem earlyExtraPC3926 : Artifact.submissionArtifact.instructionPC 3582 = 4745 := by
+@[simp] theorem earlyExtraPC3926 : Artifact.submissionArtifact.instructionPC 3579 = 4755 := by
   rw [Challenge.Modexp.Submission.Proofs.Bytecode.PCFast.instructionPC_eq_byteLength]
   rfl
 
-@[simp] theorem earlyExtraPC3927 : Artifact.submissionArtifact.instructionPC 3583 = 4746 := by
+@[simp] theorem earlyExtraPC3927 : Artifact.submissionArtifact.instructionPC 3580 = 4756 := by
   rw [Challenge.Modexp.Submission.Proofs.Bytecode.PCFast.instructionPC_eq_byteLength]
   rfl
 
-@[simp] theorem earlyExtraPC3928 : Artifact.submissionArtifact.instructionPC 3584 = 4747 := by
+@[simp] theorem earlyExtraPC3928 : Artifact.submissionArtifact.instructionPC 3581 = 4757 := by
   rw [Challenge.Modexp.Submission.Proofs.Bytecode.PCFast.instructionPC_eq_byteLength]
   rfl
 
